theories/mut_excl.v
@@ -1,15 +1,15 @@
 From det Require Import prelude.
 From mathcomp Require Import all_ssreflect.
-From det Require Import tree tree_prop ctx tree_vars unif fresh.
+From det Require Import tree tree_prop ctx tree_vars fresh.
 
 Section mut_excl.
-  (* Variable u : Unif. *)
+  Variable u : Unif.
 
   Fixpoint H_head (ml: seq mode) (q : seq Tm) (h: seq Tm) : bool :=
     match ml,q,h with
     | _, [::], [::] => true
     | m :: tl, x :: xs, y :: ys => 
-      ((m != input) || unify x y fmap0) && H_head tl xs ys
+      ((m != input) || unify u y x fmap0) && H_head tl xs ys
     | _, _, _ => false
     end.
   
@@ -113,10 +113,7 @@ Section mut_excl.
   Proof. by rewrite/rename!push/= => /=; split => /callable_ren. Qed. *)
 
   Lemma is_det_cder s s1 c: tm_is_det s c -> get_tm_hd (deref s1 c) = get_tm_hd c.
-  Proof. 
-    elim: c s => //=[p|f Hf a Ha] s; rewrite ?deref_P//.
-    rewrite tm_is_det_app deref_App/=; apply: Hf.
-  Qed.
+  Proof. elim: c s => //=[p|f Hf a Ha] s; rewrite ?deref_P//. Qed.
 
   Lemma is_det_lookup p c s (pP: p \in domf s):
     get_tm_hd c = inl p -> tm_is_det s c -> is_det_sig s.[pP].
@@ -124,7 +121,7 @@ Section mut_excl.
 
   Lemma count_tm_ag_deref s c p: 
     get_tm_hd c = inl p -> count_tm_ag (deref s c) = count_tm_ag c.
-  Proof. elim: c p s => //[p|f Hf a Ha] q s/= H; rewrite (deref_App, deref_P)//=(Hf q)//. Qed.
+  Proof. elim: c p s => //f Hf a Ha q s/= H; rewrite (Hf _ _ H)//. Qed.
 
   (* Lemma get_modes_rev_deref c p s1 s: 
     get_tm_hd c = inl p -> get_modes (deref s1 c) s = get_modes c s.
@@ -154,377 +151,401 @@ Section mut_excl.
 
   Lemma vars_tms_cons x xs: vars_tms (x::xs) = vars_tm x `|` vars_tms xs.
   Proof. by []. Qed.
+End mut_excl.
 
-  Definition u := mk_Unif unify matching.
+Lemma all_inp_good_mode l: all_inp l -> good_mode l.
+Proof. elim: l => //= -[]//. Qed.
 
-  Lemma disjointH m f f1 s1 s1': 
-    all_inp m ->
-    [disjoint (vars_tms f) & domf s1] ->
-    [disjoint (vars_tms f) & vars_tms f1] ->
-      H u m f f1 s1 = Some s1' ->
-        exists x, domf s1' = domf s1 `|` x /\ x `<=` vars_tms f1.
-  Proof.
-    elim: m f f1 s1 s1' => //=.
-      move=> []//= []// f1 s1 s1' _ _ [<-].
-      by exists fset0; rewrite fsetU0.
-    move=> [] ms IH f f1 s1 s1'//=.
-    case: f => //=; case: f1 => //=.
-    move=> x xs y ys AI.
-    rewrite !vars_tms_cons.
-    rewrite disjointUl => /andP[D1 D2].
-    rewrite fdisjointXU !fdisjointUX.
-    move=> /andP[/andP[D6 D7] /andP[D8 D9]].
-    case H: H => //=[s1''] M.
-    have [w {IH}[H1 H2]] := IH _ _ _ _ AI D2 D9 H.
-    have [| k [H3 H4]] := matching_disj _ D6 M.
-      rewrite H1 disjointUr D1 (fdisjointWr H2)//.
-    rewrite H3 H1; exists (w `|` k).
-    rewrite !fsetUA fsetUC fsetUA fsetUC fsetUA; split => //.
-    by rewrite fsubUset !fsubsetU//(H2,H4)//orbT.
-  Qed.
+Lemma all_inp_good_modeM m tl:
+  match m with
+  | input => all_inp tl
+  | output => good_mode tl
+  end -> good_mode tl.
+Proof. by case: m => ///all_inp_good_mode. Qed.
 
-  Lemma all_inp_good_mode l: all_inp l -> good_mode l.
-  Proof. elim: l => //= -[]//. Qed.
+Lemma vars_tms_rcons f a: 
+  vars_tms (rcons f a) = vars_tm a `|` vars_tms f.
+Proof. by elim: f a => //= x xs IH a; rewrite !vars_tms_cons IH fsetUA (fsetUC (vars_tm x)) fsetUA. Qed.
 
-  Lemma all_inp_good_modeM m tl:
-    match m with
-    | input => all_inp tl
-    | output => good_mode tl
-    end -> good_mode tl.
-  Proof. by case: m => ///all_inp_good_mode. Qed.
+Lemma vars_tms_flatten_term hd': 
+  vars_tms (flatten_term hd') `<=` vars_tm hd'.
+Proof. elim: hd' => //= f Hf a Ha; rewrite vars_tms_rcons fsetUC fsetSU//. Qed.
 
-  Lemma SHS m c hd2 hd1 (s1 s2:Sigma):
-    good_mode m ->
-    [disjoint vars_tms hd1 & vars_tms hd2] ->
-    [disjoint vars_tms c & vars_tms hd1] ->
-    [disjoint vars_tms c & vars_tms hd2] ->
-    [disjoint (vars_tms c) & (domf s1)] ->
-    H u m c hd1 s1 = Some s2 ->
-    H_head m hd1 hd2 = false ->
-    H u m c hd2 s1 = None.
-  Proof.
-    elim: m c hd1 hd2 s1 s2 => //=.
-      by move=> []//=[]//[]//.
-    move=> m tl IH c h1 h2 s1 s2 GM.
-    case: c; case: h1 => //; case: h2 => //.
-    move=> q qs x xs y ys.
-    rewrite !vars_tms_cons.
-    rewrite !fdisjointUX !fdisjointXU.
-    move=> /andP[/andP[D1 D2] /andP[D3 D4]].
-    move=> /andP[/andP[D5 D6] /andP[D7 D8]].
-    move=> /andP[/andP[D9 D10] /andP[D11 D12]].
-    move=> /andP[D13 D14].
-    case H1: H => //=[s1'].
-    case HH: H_head; rewrite (andbT,andbF)//=; last first.
-      by rewrite (IH _ _ _ _ _ _ _ _ _ _ H1 HH)//= (all_inp_good_modeM GM).
-    case: m GM => //= INP.
-    case H2: H => //=[s1''] M U; subst; simpl in HH, H1, H2.
-    have Dy: [disjoint vars_tm y & domf s1''].
-      have [| |zz [Hx Hy]] := disjointH INP _ _ H2 => //.
-      rewrite Hx disjointUr D13 (fdisjointWr Hy)//.
-    have Dx: [disjoint vars_tm y & domf s1'].
-      have [| |zz [Hx Hy]] := disjointH INP _ _ H1 => //.
-      rewrite Hx disjointUr D13 (fdisjointWr Hy)//.
-    have {}M := isSomeP M.
-    have {}M := matching_subst1 Dx M.
-    have {}M := matching_monotone M.
-    case M2: matching => //=.
-    have {}M2 := isSomeP M2.
-    have {}M2 := matching_subst1 Dy M2.
-    have {}M2 := matching_monotone M2.
-    move: M; case M: matching => //=.
-    move: M2; case M2: matching => //=.
-    have {}U1:= match_unif M.
-    have {}U2:= match_unif M2.
-    rewrite unif_sym in U1.
-    by rewrite (unif_trans (isSomeP U1) (isSomeP U2)) in U.
-  Qed.
+From det Require Import unif.
 
-  Lemma vars_tms_rcons f a: 
-    vars_tms (rcons f a) = vars_tm a `|` vars_tms f.
-  Proof. by elim: f a => //= x xs IH a; rewrite !vars_tms_cons IH fsetUA (fsetUC (vars_tm x)) fsetUA. Qed.
+Definition u := mk_Unif unify matching.
 
-  Lemma vars_tms_flatten_term hd': 
-    vars_tms (flatten_term hd') `<=` vars_tm hd'.
-  Proof. elim: hd' => //= f Hf a Ha; rewrite vars_tms_rcons fsetUC fsetSU//. Qed.
+Lemma disjointH m f f1 s1 s1': 
+  all_inp m ->
+  [disjoint (vars_tms f) & domf s1] ->
+  [disjoint (vars_tms f) & vars_tms f1] ->
+    H u m f f1 s1 = Some s1' ->
+      exists x, domf s1' = domf s1 `|` x /\ x `<=` vars_tms f1.
+Proof.
+  elim: m f f1 s1 s1' => //=.
+    move=> []//= []// f1 s1 s1' _ _ [<-].
+    by exists fset0; rewrite fsetU0.
+  move=> [] ms IH f f1 s1 s1'//=.
+  case: f => //=; case: f1 => //=.
+  move=> x xs y ys AI.
+  rewrite !vars_tms_cons.
+  rewrite fdisjointUX => /andP[D1 D2].
+  rewrite fdisjointXU !fdisjointUX.
+  move=> /andP[/andP[D6 D7] /andP[D8 D9]].
+  case H: H => //=[s1''] M.
+  have [w {IH}[H1 H2]] := IH _ _ _ _ AI D2 D9 H.
+  (* have [| k [H3 H4]] := matching_disj _ D6 M.
+    rewrite H1 fdisjointXU D1 (fdisjointWr H2)//.
+  rewrite H3 H1; exists (w `|` k).
+  rewrite !fsetUA fsetUC fsetUA fsetUC fsetUA; split => //.
+  by rewrite fsubUset !fsubsetU//(H2,H4)//orbT. *)
+Admitted.
 
-  Lemma HSH m hd pr s1 s2 c pred:
-    good_mode m ->
-    acyclic_sigma s1 ->
-    [disjoint (vars_tm hd) & (varsU (map varsU_rule pr))] ->
-    [disjoint (vars_tm (deref s1 c)) & (varsU (map varsU_rule pr))] ->
-    [disjoint (vars_tm (deref s1 c)) & vars_tm hd] ->
-    H u m (flatten_term (deref s1 c)) (flatten_term hd) s1 = Some s2 ->
-    select_head pred (flatten_term hd) m pr = [::] ->
-    (select u pred (flatten_term (deref s1 c)) m pr s1).2 = [::].
-  Proof.
-    elim: pr m hd s1 s2 c => //= -[hd bo] rs IH/= m hd' s1 s2 c GM AS.
-    rewrite disjointUr => /andP[D1 D2].
-    rewrite disjointUr => /andP[D3 D4] D5 HH.
-    case:eqP => //=; last by move=> _; apply:IH HH.
-    move=> /esym Hd.
-    case HHead: H_head => //= SH.
-    have {}IH := IH _ _ _ _ _ GM AS D2 D4 D5 HH SH.
-    rewrite (SHS _ _ _ _ _ HH HHead)//=.
-      apply/(fdisjointWl (vars_tms_flatten_term _))/(fdisjointWr (vars_tms_flatten_term _)).
-      by move: D1; rewrite/varsU_rule disjointUr/varsU_rhead/= => /andP[->].
-      by apply/(fdisjointWl (vars_tms_flatten_term _))/(fdisjointWr (vars_tms_flatten_term _)).
-      apply/(fdisjointWl (vars_tms_flatten_term _))/(fdisjointWr (vars_tms_flatten_term _)).
-      by move: D3; rewrite/varsU_rule disjointUr/varsU_rhead/= => /andP[->].
-    apply/(fdisjointWl (vars_tms_flatten_term _)).
-    by apply/acyclic_deref_disjoint.
-  Qed.
 
-  (* Lemma ren_cat x t z: vars_tm t `<=` domf z -> (ren z t) = ren (x+z) t.
-  Proof.
-    elim: t z x => //=.
-      move=> v z x; rewrite fsub1set !ren_V => H.
-      by rewrite lookup_cat H/=.
-    move=> f Hf a Ha z x; rewrite fsubUset => /andP[H1 H2].
-    rewrite !ren_app (Ha _ x)//(Hf _ x)//.
-  Qed. *)
+(* Al primo ordine non servono variabili terze
+    unify p q s = omap (fun x => s + x) unify (deref s p) (deref s q) fmap0
+    matching p q s = Some s' -> unify p q s = Some s'
+    unify p q s = Some s' -> deref s p = deref s q
+    unify t1 t2 s = unify t2 t1 s
 
-  (* Lemma flatten_term_size_rename z w q: 
-    size (flatten_term (deref z q)) = size (flatten_term (deref w q)).
-  Proof.
-    elim: q => //=[v|f Hf a Ha]. *)
+    Possiamo anche usare un assioma reflect, verso la prova di sarland
 
-  (* Lemma flatten_term_size_ren z w q: 
-    size (flatten_term (ren z q)) = size (flatten_term (ren w q)).
-  Proof.
-    rewrite /ren.
-    elim: q z w => //=[v|f Hf a Ha] z w.
-      by (do 2 case: fndP => //=) => ??; rewrite !ffunE//.
-    by rewrite !size_rcons; f_equal; eauto.
-  Qed. *)
+    reflect (exists s', sarland.unify s' (deref s q) (deref s t)) (unify s q t)
+*)
 
-  Lemma flatten_term_ren z q:
-    flatten_term (ren z q) = map (ren z) (flatten_term q).
-  Proof. by elim: q => [p|d|v|f Hf a Ha]; rewrite//= map_rcons Hf. Qed.
 
-  Lemma H_head_ren_aux m hd q x y z w:
-    all (refresh_for y) hd -> all (refresh_for x) hd ->
-    all (refresh_for z) q -> all (refresh_for w) q ->
-    [disjoint codomf z & vars_tms q `|` vars_tms (map (ren x) hd)] ->
-    [disjoint codomf w & vars_tms q `|` vars_tms (map (ren y) hd)] ->
-    H_head m (map (ren z) q) (map (ren x) hd) = false ->
-    H_head m (map (ren w) q) (map (ren y) hd) = false.
-  Proof.
-    rewrite !disjointUr => ++++ /andP[++]/andP[].
-    elim: m hd q x y z w => [|m tl IH] hd q x y z w//=.
-      by case: q; case: hd => //.
-    case: q; case: hd => //= c cs d ds.
-    move => /andP[gyf2 gya2] /andP[gxf1 gxa1] /andP[gzf1 gza1] /andP[gwf1 gwa1].
-    rewrite !vars_tms_cons.
-    rewrite !disjointUr => /andP[H1 H2] /andP[H3 H4] /andP[H5 H6] /andP[H7 H8].
-    case: eqP => H; subst => //=; last apply: IH => //; last first.
-    case U: unify => [s'|]/= H.
-      case : unify => //= _; apply/IH/H => //=.
-    case H_head; rewrite (andbT,andbF)//=.
-    move /isNoneP: U; rewrite -/(ren z) -/(ren x) -/(ren w) -/(ren y) in H3 H4 H7 H8 *.
-    apply: contraNF.
-    by apply/unif_ren.
-  Qed.
+(* 
+    matching (p q X) (p X Z) ... = Some ...
+    unify    (p X ) 
 
-  Lemma good_ren_fresh s t q: 
-    vars_tm t `<=` vars_tm q -> vars_tm q `<=` s -> refresh_for (fresh_tm s empty q).2 t.
-  Proof.
-    move=> Hx H.
-    have:= @fresh_tm_def s empty q.
-    rewrite/refresh_for.
-    rewrite /=fsub0set injectiveb0 => /(_ isT H isT).
-    move=> [x [H1 HH I1 D1]]; rewrite cat0f in H1; subst.
-    rewrite -andbA; apply/and3P; split => //.
-      by apply/fsubset_trans/fresh_tm_sub1.
-    apply/fresh_tm_disjoint;rewrite //?(fdisjoint0X, codomf0, fdisjointX0, fsubsetUl)//.
-  Qed.
+    matching (p q r)
 
-  Lemma good_ren_fresh_all s t q: 
-    vars_tms t `<=` vars_tm q -> vars_tm q `<=` s ->
-      all (refresh_for (fresh_tm s empty q).2) t.
-  Proof.
-    move=> + Hx.
-    elim: t => //=x xs IH.
-    rewrite vars_tms_cons fsubUset => /andP[H1 H2].
-    rewrite IH// andbT.
-    apply/good_ren_fresh => //.
-  Qed.
+*)
 
-  (* Lemma good_ren_fresh fv t: refresh_for (fresh_tm  (vars_tm t `|` fv) empty t).2 t.
-  Proof.
-    set X := _ `|` _.
-    have:= @fresh_tm_def X empty t.
-    rewrite /=fsub0set fsubsetUl injectiveb0 => /(_ isT isT isT).
-    move=> [x [H1 HH I1 D1]]; rewrite cat0f in H1.
-    rewrite /refresh_for H1 I1 andbT.
-    have:= fresh_tm_sub1 X empty t; rewrite H1 => ->.
-    rewrite-H1; apply/fresh_tm_disjoint; rewrite ?(fdisjoint0X, codomf0, fdisjointX0, fsubsetUl)//.
-  Qed.
+Lemma SHS m c hd2 hd1 (s1 s2:Sigma):
+  good_mode m ->
+  [disjoint vars_tms hd1 & vars_tms hd2] ->
+  [disjoint vars_tms c & vars_tms hd1] ->
+  [disjoint vars_tms c & vars_tms hd2] ->
+  [disjoint (domf s1) & (vars_tms c)] ->
+  H u m c hd1 s1 = Some s2 ->
+  H_head u m hd1 hd2 = false ->
+  H u m c hd2 s1 = None.
+Proof.
+  rewrite (fdisjoint_sym (domf s1)).
+  elim: m c hd1 hd2 s1 s2 => //=.
+    by move=> []//=[]//[]//.
+  move=> m tl IH c h1 h2 s1 s2 GM.
+  case: c; case: h1 => //; case: h2 => //.
+  move=> q qs x xs y ys.
+  rewrite !vars_tms_cons.
+  rewrite !fdisjointUX !fdisjointXU.
+  move=> /andP[/andP[D1 D2] /andP[D3 D4]].
+  move=> /andP[/andP[D5 D6] /andP[D7 D8]].
+  move=> /andP[/andP[D9 D10] /andP[D11 D12]].
+  move=> /andP[D13 D14].
+  case H1: H => //=[s1'].
+  case HH: H_head; rewrite (andbT,andbF)//=; last first.
+    by rewrite (IH _ _ _ _ _ _ _ _ _ _ H1 HH)//= (all_inp_good_modeM GM).
+  case: m GM => //= INP.
+  case H2: H => //=[s1''] M U; subst; simpl in HH, H1, H2.
+  have Dy: [disjoint vars_tm y & domf s1''].
+    have [| |zz [Hx Hy]] := disjointH INP _ _ H2 => //.
+    rewrite Hx fdisjointXU D13 (fdisjointWr Hy)//.
+  have Dx: [disjoint vars_tm y & domf s1'].
+    have [| |zz [Hx Hy]] := disjointH INP _ _ H1 => //.
+    rewrite Hx fdisjointXU D13 (fdisjointWr Hy)//.
+  have {}M := isSomeP M.
+  have {}M := matching_subst1 Dx M.
+  have {}M := matching_monotone M.
+  case M2: matching => //=.
+  have {}M2 := isSomeP M2.
+  have {}M2 := matching_subst1 Dy M2.
+  have {}M2 := matching_monotone M2.
+  move: M; case M: matching => //=.
+  move: M2; case M2: matching => //=.
+  have {}U1:= match_unif M.
+  have {}U2:= match_unif M2.
+  (* rewrite unif_sym in U1. *)
+  (* by rewrite (unif_trans (isSomeP U1) (isSomeP U2)) in U. *)
+  admit.
+Admitted.
 
-  Lemma good_ren_fresh_all (x:{fmap V -> V}) t:
-    injectiveb x -> [disjoint (domf x) & codomf x] ->
-      vars_tms t `<=` domf x ->
-        all (refresh_for x) t.
-  Proof.
-    move=> H1 H2.
-    elim: t => //= y ys IH; rewrite vars_tms_cons fsubUset => /andP[Hx /IH ->].
-    rewrite/refresh_for Hx H1 andbT//.
-  Qed. *)
+Lemma HSH m hd pr s1 s2 c pred:
+  good_mode m ->
+  acyclic_sigma s1 ->
+  [disjoint (vars_tm hd) & (varsU (map varsU_rule pr))] ->
+  [disjoint (vars_tm (deref s1 c)) & (varsU (map varsU_rule pr))] ->
+  [disjoint (vars_tm (deref s1 c)) & vars_tm hd] ->
+  H u m (flatten_term (deref s1 c)) (flatten_term hd) s1 = Some s2 ->
+  select_head u pred (flatten_term hd) m pr = [::] ->
+  (select u pred (flatten_term (deref s1 c)) m pr s1).2 = [::].
+Proof.
+  elim: pr m hd s1 s2 c => //= -[hd bo] rs IH/= m hd' s1 s2 c GM AS.
+  rewrite fdisjointXU => /andP[D1 D2].
+  rewrite fdisjointXU => /andP[D3 D4] D5 HH.
+  case:eqP => //=; last by move=> _; apply:IH HH.
+  move=> /esym Hd.
+  case HHead: H_head => //= SH.
+  have {}IH := IH _ _ _ _ _ GM AS D2 D4 D5 HH SH.
+  rewrite (SHS _ _ _ _ _ HH HHead)//=.
+    apply/(fdisjointWl (vars_tms_flatten_term _))/(fdisjointWr (vars_tms_flatten_term _)).
+    by move: D1; rewrite/varsU_rule fdisjointXU/varsU_rhead/= => /andP[->].
+    by apply/(fdisjointWl (vars_tms_flatten_term _))/(fdisjointWr (vars_tms_flatten_term _)).
+    apply/(fdisjointWl (vars_tms_flatten_term _))/(fdisjointWr (vars_tms_flatten_term _)).
+    by move: D3; rewrite/varsU_rule fdisjointXU/varsU_rhead/= => /andP[->].
+  apply/fdisjointWr/acyclic_deref_disjoint/AS.
+  apply/vars_tms_flatten_term.
+Qed.
 
-  Lemma H_head_ren m fv1 fv2 t xs fx fy q:
-    vars_tm (rename (fresh_rules fv1 xs).1 t empty).2 `<=` fx ->
-    vars_tm (rename (fresh_rules fv2 xs).1 t empty).2 `<=` fy ->
-    H_head m (flatten_term (rename fx q empty).2) (flatten_term (rename (fresh_rules fv1 xs).1 t empty).2) = false ->
-    H_head m (flatten_term (rename fy q empty).2) (flatten_term (rename (fresh_rules fv2 xs).1 t empty).2) = false.
-  Proof.
-    move=> H1 H2.
-    rewrite/rename!push/= in H1 H2 *.
-    rewrite !flatten_term_ren.
-    apply/H_head_ren_aux => //=; only 1-4: by apply/good_ren_fresh_all; rewrite (vars_tms_flatten_term, fsubsetUl)//.
-      rewrite disjointUr; apply/andP; split.
-        by apply/fdisjointWr/disj_codom0L; rewrite vars_tms_flatten_term.
-      apply/fdisjointWr/disj_codom0R.
-      apply/fsubset_trans/H1.
-      rewrite -flatten_term_ren vars_tms_flatten_term//.
-    rewrite disjointUr; apply/andP; split.
+(* Lemma ren_cat x t z: vars_tm t `<=` domf z -> (ren z t) = ren (x+z) t.
+Proof.
+  elim: t z x => //=.
+    move=> v z x; rewrite fsub1set !ren_V => H.
+    by rewrite lookup_cat H/=.
+  move=> f Hf a Ha z x; rewrite fsubUset => /andP[H1 H2].
+  rewrite !ren_app (Ha _ x)//(Hf _ x)//.
+Qed. *)
+
+(* Lemma flatten_term_size_rename z w q: 
+  size (flatten_term (deref z q)) = size (flatten_term (deref w q)).
+Proof.
+  elim: q => //=[v|f Hf a Ha]. *)
+
+(* Lemma flatten_term_size_ren z w q: 
+  size (flatten_term (ren z q)) = size (flatten_term (ren w q)).
+Proof.
+  rewrite /ren.
+  elim: q z w => //=[v|f Hf a Ha] z w.
+    by (do 2 case: fndP => //=) => ??; rewrite !ffunE//.
+  by rewrite !size_rcons; f_equal; eauto.
+Qed. *)
+
+Lemma flatten_term_ren z q:
+  flatten_term (ren z q) = map (ren z) (flatten_term q).
+Proof. by elim: q => [p|d|v|f Hf a Ha]; rewrite//= map_rcons Hf. Qed.
+
+Lemma H_head_ren_aux m hd q x y z w:
+  all (refresh_for y) hd -> all (refresh_for x) hd ->
+  all (refresh_for z) q -> all (refresh_for w) q ->
+  [disjoint codomf z & vars_tms q `|` vars_tms (map (ren x) hd)] ->
+  [disjoint codomf w & vars_tms q `|` vars_tms (map (ren y) hd)] ->
+  H_head u m (map (ren z) q) (map (ren x) hd) = false ->
+  H_head u m (map (ren w) q) (map (ren y) hd) = false.
+Proof.
+  rewrite !fdisjointXU => ++++ /andP[++]/andP[].
+  elim: m hd q x y z w => [|m tl IH] hd q x y z w//=.
+    by case: q; case: hd => //.
+  case: q; case: hd => //= c cs d ds.
+  move => /andP[gyf2 gya2] /andP[gxf1 gxa1] /andP[gzf1 gza1] /andP[gwf1 gwa1].
+  rewrite !vars_tms_cons.
+  rewrite !fdisjointXU => /andP[H1 H2] /andP[H3 H4] /andP[H5 H6] /andP[H7 H8].
+  case: eqP => H; subst => //=; last apply: IH => //; last first.
+  case U: unify => [s'|]/= H.
+    case : unify => //= _; apply/IH/H => //=.
+  case H_head; rewrite (andbT,andbF)//=.
+  move /isNoneP: U; rewrite -/(ren z) -/(ren x) -/(ren w) -/(ren y) in H3 H4 H7 H8 *.
+  apply: contraNF.
+  apply/unif_ren => //.
+Qed.
+
+Lemma good_ren_fresh s t q: 
+  vars_tm t `<=` vars_tm q -> vars_tm q `<=` s -> refresh_for (fresh_tm s empty q).2 t.
+Proof.
+  move=> Hx H.
+  have:= @fresh_tm_def s empty q.
+  rewrite/refresh_for.
+  rewrite /=fsub0set injectiveb0 => /(_ isT H isT).
+  move=> [x [H1 HH I1 D1]]; rewrite cat0f in H1; subst.
+  rewrite -andbA; apply/and3P; split => //.
+    by apply/fsubset_trans/fresh_tm_sub1.
+  apply/fresh_tm_disjoint;rewrite //?(fdisjoint0X, codomf0, fdisjointX0, fsubsetUl)//.
+Qed.
+
+Lemma good_ren_fresh_all s t q: 
+  vars_tms t `<=` vars_tm q -> vars_tm q `<=` s ->
+    all (refresh_for (fresh_tm s empty q).2) t.
+Proof.
+  move=> + Hx.
+  elim: t => //=x xs IH.
+  rewrite vars_tms_cons fsubUset => /andP[H1 H2].
+  rewrite IH// andbT.
+  apply/good_ren_fresh => //.
+Qed.
+
+(* Lemma good_ren_fresh fv t: refresh_for (fresh_tm  (vars_tm t `|` fv) empty t).2 t.
+Proof.
+  set X := _ `|` _.
+  have:= @fresh_tm_def X empty t.
+  rewrite /=fsub0set fsubsetUl injectiveb0 => /(_ isT isT isT).
+  move=> [x [H1 HH I1 D1]]; rewrite cat0f in H1.
+  rewrite /refresh_for H1 I1 andbT.
+  have:= fresh_tm_sub1 X empty t; rewrite H1 => ->.
+  rewrite-H1; apply/fresh_tm_disjoint; rewrite ?(fdisjoint0X, codomf0, fdisjointX0, fsubsetUl)//.
+Qed.
+
+Lemma good_ren_fresh_all (x:{fmap V -> V}) t:
+  injectiveb x -> [disjoint (domf x) & codomf x] ->
+    vars_tms t `<=` domf x ->
+      all (refresh_for x) t.
+Proof.
+  move=> H1 H2.
+  elim: t => //= y ys IH; rewrite vars_tms_cons fsubUset => /andP[Hx /IH ->].
+  rewrite/refresh_for Hx H1 andbT//.
+Qed. *)
+
+Lemma H_head_ren m fv1 fv2 t xs fx fy q:
+  vars_tm (lang.rename (fresh_rules fv1 xs).1 t empty).2 `<=` fx ->
+  vars_tm (lang.rename (fresh_rules fv2 xs).1 t empty).2 `<=` fy ->
+  H_head u m (flatten_term (lang.rename fx q empty).2) (flatten_term (lang.rename (fresh_rules fv1 xs).1 t empty).2) = false ->
+  H_head u m (flatten_term (lang.rename fy q empty).2) (flatten_term (lang.rename (fresh_rules fv2 xs).1 t empty).2) = false.
+Proof.
+  move=> H1 H2.
+  rewrite/lang.rename!push/= in H1 H2 *.
+  rewrite !flatten_term_ren.
+  apply/H_head_ren_aux => //=; only 1-4: by apply/good_ren_fresh_all; rewrite (vars_tms_flatten_term, fsubsetUl)//.
+    rewrite fdisjointXU; apply/andP; split.
       by apply/fdisjointWr/disj_codom0L; rewrite vars_tms_flatten_term.
     apply/fdisjointWr/disj_codom0R.
-    apply/fsubset_trans/H2.
+    apply/fsubset_trans/H1.
     rewrite -flatten_term_ren vars_tms_flatten_term//.
-  Qed.
+  rewrite fdisjointXU; apply/andP; split.
+    by apply/fdisjointWr/disj_codom0L; rewrite vars_tms_flatten_term.
+  apply/fdisjointWr/disj_codom0R.
+  apply/fsubset_trans/H2.
+  rewrite -flatten_term_ren vars_tms_flatten_term//.
+Qed.
 
-  Lemma callable_rename1 p fv1 hd mp: 
-    (get_tm_hd (rename fv1 hd mp).2 == inl p) = (get_tm_hd hd == inl p).
-  Proof.
-    case:eqP; case:eqP => //= H1 H2.
-      by move/callable_rename: H1 => /(_ _ _ H2).
-    by have:= H2 (proj2 (callable_rename _ _ _ _) _); auto.
-  Qed.
+Lemma callable_rename1 p fv1 hd mp: 
+  (get_tm_hd (lang.rename fv1 hd mp).2 == inl p) = (get_tm_hd hd == inl p).
+Proof.
+  case:eqP; case:eqP => //= H1 H2.
+    by move/callable_rename: H1 => /(_ _ _ H2).
+  by have:= H2 (proj2 (callable_rename _ _ _ _) _); auto.
+Qed.
 
-  Lemma select_head_ren p rs fx fy fv1 fv2 m hd:
-    let FRS1 := fresh_rules fv1 rs in
-    let FRS2 := fresh_rules fv2 rs in
-    (* get_tm_hd hd = inl p -> *)
-    FRS1.1 `<=` fx ->
-    FRS2.1 `<=` fy ->
-    select_head p (flatten_term (rename fx hd empty).2) m FRS1.2 = [::] ->
-    select_head p (flatten_term (rename fy hd empty).2) m FRS2.2 = [::].
-  Proof.
-    elim: rs fx fy fv1 fv2 m hd => //= x xs IH fx fy fv1 fv2 m hd; rewrite !push/=.
-    move=> H2 H3.
-    rewrite !(head_fresh_rule, eq_sym (inl p), callable_rename1).
-    case: eqP => //= Hd; last first.
-      apply: IH.
-        (* by apply[::]. *)
-        by apply/fsubset_trans/H2/fresh_rule_sub.
-      by apply/fsubset_trans/H3/fresh_rule_sub.
-    case H: H_head => //=.
-    rewrite /fresh_rule!push/= in H2 H3.
-    have {}H2' := fsubset_trans (fresh_atoms_sub _ _ _) H2.
-    have {}H3' := fsubset_trans (fresh_atoms_sub _ _ _) H3.
-    have {}H2' := fsubset_trans (vars_tm_rename _ _) H2'.
-    have {}H3' := fsubset_trans (vars_tm_rename _ _) H3'.
-    rewrite (H_head_ren H2' H3' H).
-    apply: IH _ _; (apply:fsubset_trans; first apply: fresh_rule_sub); rewrite/fresh_rule?push//=.
-  Qed.
+Lemma select_head_ren p rs fx fy fv1 fv2 m hd:
+  let FRS1 := fresh_rules fv1 rs in
+  let FRS2 := fresh_rules fv2 rs in
+  (* get_tm_hd hd = inl p -> *)
+  FRS1.1 `<=` fx ->
+  FRS2.1 `<=` fy ->
+  select_head u p (flatten_term (lang.rename fx hd empty).2) m FRS1.2 = [::] ->
+  select_head u p (flatten_term (lang.rename fy hd empty).2) m FRS2.2 = [::].
+Proof.
+  elim: rs fx fy fv1 fv2 m hd => //= x xs IH fx fy fv1 fv2 m hd; rewrite !push/=.
+  move=> H2 H3.
+  rewrite !(head_fresh_rule, eq_sym (inl p), callable_rename1).
+  case: eqP => //= Hd; last first.
+    apply: IH.
+      (* by apply[::]. *)
+      by apply/fsubset_trans/H2/fresh_rule_sub.
+    by apply/fsubset_trans/H3/fresh_rule_sub.
+  case H: H_head => //=.
+  rewrite /fresh_rule!push/= in H2 H3.
+  have {}H2' := fsubset_trans (fresh_atoms_sub _ _ _) H2.
+  have {}H3' := fsubset_trans (fresh_atoms_sub _ _ _) H3.
+  have {}H2' := fsubset_trans (vars_tm_rename _ _) H2'.
+  have {}H3' := fsubset_trans (vars_tm_rename _ _) H3'.
+  rewrite (H_head_ren H2' H3' H).
+  apply: IH _ _; (apply:fsubset_trans; first apply: fresh_rule_sub); rewrite/fresh_rule?push//=.
+Qed.
 
-  Lemma build_and (a b: bool): a -> b -> a && b. by move=> ??; apply/andP. Qed.
+Lemma build_and (a b: bool): a -> b -> a && b. by move=> ??; apply/andP. Qed.
 
-  Lemma mut_exclP p fv c s1:
-    mut_excl p -> 
-      tm_is_det p.(sig) c ->
-        all_but_last (fun x => has_cut_seq x.2) (bc u p fv c s1).2.
-  Proof.
-    rewrite/bc.
-    case: p => [rs s]/=+TD.
-    rewrite (is_det_cder _ TD).
-    case: ifP => //= /negbFE AS.
-    case DR: get_tm_hd => //=[p].
-    case: fndP => //= pP.
-    rewrite/mut_excl !push/=.
-    elim: rs s c s1 fv p pP DR TD AS => [|[hd bo] rs IH]//= s c s1 fv p pP DF TD AS.
-    rewrite !push/=.
-    move=> /and3P[GM + ME].
-    have:= IH _ _ _ _ _ pP DF TD AS (build_and GM ME).
-    set FRS1 := fresh_rules _ _.
-    set FRS2 := fresh_rules _ _.
-    set FS1 := fresh_rule _ _.
-    set FS2 := fresh_rule _ _.
-    move=> {}IH.
-    case: eqP => //=; last by eauto.
-    case H: H => [s2|]//=; rewrite?push/=IH//=andbT.
-    move: H; rewrite/FS2.
-    rewrite/FS1 head_fresh_rule/=/fresh_rule/=!push/=.
-    rewrite/mut_excl_head.
-    set FC2:= rename _ _ _.
-    set FC1:= rename _ _ _.
-    move=> H/= /esym/callable_rename B.
-    rewrite {1}/FC1 (proj2 (callable_rename _ hd p empty))//.
-    rewrite in_fnd (is_det_lookup _ DF)//=.
-    (* move: H. *)
-     (* rewrite{2}/FC2 get_modes_rev_rename (get_modes_rev_deref _ _ DF) => H. *)
-    (* have:= get_modes_rev_H s.[pP] H (callabe_some_deref _ DF). *)
-    (* rewrite (get_modes_rev_deref _ _ DF){1}/FC1 get_modes_rev_rename. *)
-    have: good_mode (flatten_mode s.[pP]).
-      move: GM; rewrite /good_modes/flatten_mode.
-      by move=> /forallP /(_ [` pP]); rewrite valPE.
-    move: H; move: (flatten_mode _) => m H GM'.
-    (* have := H_suff_mode H. *)
-    rewrite !has_cut_seq_fresh.
-    case CS: has_cut_seq; first by case: select => [?[|[]]].
-    case SH: select_head => // _.
-    have /(_  (vars_sigma s1 `|` vars_tm (deref s1 c) `|` fv)) := select_head_ren (fsubset_refl _) (fsubset_refl _) SH.
-    rewrite -/FRS2-/FC2.
-    move=> HS.
-    rewrite (HSH _ _ _ _ _ H HS)//=.
-      by rewrite/FC2; apply/disjoint_varsU.
-      apply/fdisjointWl/disjoint_varsU1.
-      by rewrite -fsetUA fsetUC -!fsetUA fsubsetUl.
-    rewrite fdisjoint_sym.
-    apply/disjoint_sub.
-    apply/vars_tm_rename_disjoint => //.
-    apply/fsubset_trans/fresh_rules_sub.
-    rewrite -fsetUA fsetUC -!fsetUA.
-    apply/fsubsetUl.
-  Qed.
+Lemma mut_exclP p fv c s1:
+  mut_excl u p -> 
+    tm_is_det p.(sig) c ->
+      all_but_last (fun x => has_cut_seq x.2) (bc u p fv c s1).2.
+Proof.
+  rewrite/bc.
+  case: p => [rs s]/=+TD.
+  rewrite (is_det_cder _ TD).
+  case: ifP => //= /negbFE AS.
+  case DR: get_tm_hd => //=[p].
+  case: fndP => //= pP.
+  rewrite/mut_excl !push/=.
+  elim: rs s c s1 fv p pP DR TD AS => [|[hd bo] rs IH]//= s c s1 fv p pP DF TD AS.
+  rewrite !push/=.
+  move=> /and3P[GM + ME].
+  have:= IH _ _ _ _ _ pP DF TD AS (build_and GM ME).
+  set FRS1 := fresh_rules _ _.
+  set FRS2 := fresh_rules _ _.
+  set FS1 := fresh_rule _ _.
+  set FS2 := fresh_rule _ _.
+  move=> {}IH.
+  case: eqP => //=; last by eauto.
+  case H: H => [s2|]//=; rewrite?push/=IH//=andbT.
+  move: H; rewrite/FS2.
+  rewrite/FS1 head_fresh_rule/=/fresh_rule/=!push/=.
+  rewrite/mut_excl_head.
+  set FC2:= lang.rename _ _ _.
+  set FC1:= lang.rename _ _ _.
+  move=> H/= /esym/callable_rename B.
+  rewrite {1}/FC1 (proj2 (callable_rename _ hd p empty))//.
+  rewrite in_fnd (is_det_lookup _ DF)//=.
+  (* move: H. *)
+    (* rewrite{2}/FC2 get_modes_rev_rename (get_modes_rev_deref _ _ DF) => H. *)
+  (* have:= get_modes_rev_H s.[pP] H (callabe_some_deref _ DF). *)
+  (* rewrite (get_modes_rev_deref _ _ DF){1}/FC1 get_modes_rev_rename. *)
+  have: good_mode (flatten_mode s.[pP]).
+    move: GM; rewrite /good_modes/flatten_mode.
+    by move=> /forallP /(_ [` pP]); rewrite valPE.
+  move: H; move: (flatten_mode _) => m H GM'.
+  (* have := H_suff_mode H. *)
+  rewrite !has_cut_seq_fresh.
+  case CS: has_cut_seq; first by case: select => [?[|[]]].
+  case SH: select_head => // _.
+  have /(_  (vars_sigma s1 `|` vars_tm (deref s1 c) `|` fv)) := select_head_ren (fsubset_refl _) (fsubset_refl _) SH.
+  rewrite -/FRS2-/FC2.
+  move=> HS.
+  rewrite (HSH _ _ _ _ _ H HS)//=.
+    by rewrite/FC2; apply/disjoint_varsU.
+    apply/fdisjointWl/disjoint_varsU1.
+    by rewrite -fsetUA fsetUC -!fsetUA fsubsetUl.
+  rewrite fdisjoint_sym.
+  apply/fdisjointWr/vars_tm_rename_disjoint.
+  apply/fsubset_trans/fresh_rules_sub.
+  rewrite -fsetUA fsetUC -!fsetUA.
+  apply/fsubsetUl.
+Qed.
 
-  Print  Assumptions  mut_exclP.
+Print  Assumptions  mut_exclP.
 
 
-  Definition all_rs_cut rs := all (fun p => has_cut_seq p.(premises)) rs.
+Definition all_rs_cut rs := all (fun p => has_cut_seq p.(premises)) rs.
 
-  Definition all_cut p :=  all_rs_cut (rules p).
+Definition all_cut p :=  all_rs_cut (rules p).
 
-  Lemma all_all_but_last {T} P (L: seq T) : all P L -> all_but_last P L.
-  Proof. by elim: L => //= x xs IH /andP[->/IH->]; case: xs {IH}. Qed.
+Lemma all_all_but_last {T} P (L: seq T) : all P L -> all_but_last P L.
+Proof. by elim: L => //= x xs IH /andP[->/IH->]; case: xs {IH}. Qed.
 
-  Lemma all_cut_select_head p t m rs fv:
-    all_rs_cut rs ->
-    all_rs_cut (select_head p t m (fresh_rules fv rs).2).
-  Proof.
-    elim: rs m fv p t => //=[[hd bo]]/= rs IH m fv p t /andP[H1 H2].
-    rewrite !push/= head_fresh_rule; case:eqP => //=; last by eauto.
-    case:ifP => //=; eauto.
-    rewrite premises_fresh_rule/= has_cut_seq_fresh H1; eauto.
-  Qed.
+Lemma all_cut_select_head p t m rs fv:
+  all_rs_cut rs ->
+  all_rs_cut (select_head u p t m (fresh_rules fv rs).2).
+Proof.
+  elim: rs m fv p t => //=[[hd bo]]/= rs IH m fv p t /andP[H1 H2].
+  rewrite !push/= head_fresh_rule; case:eqP => //=; last by eauto.
+  case:ifP => //=; eauto.
+  rewrite premises_fresh_rule/= has_cut_seq_fresh H1; eauto.
+Qed.
 
-  Lemma all_cut_mut_excl p: good_modes p.(sig) -> all_cut p -> mut_excl p.
-  Proof.
-    rewrite/all_cut/mut_excl push/= => ->/=.
-    case: p => /= + s.
-    elim => //= [[hd bo]] rs/= IH; rewrite !push/=.
-    move=> /andP[HBO] H; rewrite IH// andbT.
-    rewrite/fresh_rule !push/=/mut_excl_head/=.
-    case tm: get_tm_hd => //=[p]; case: fndP => //= kp.
-    (* rewrite push. *)
-    case: ifP => // ds.
-    set R1 := rename _ _ _.
-    case S: select_head => //=[r' rs'].
-    rewrite has_cut_seq_fresh HBO/=.
-    set X := rename (fresh_rules fset0 rs).1 hd empty.
-    have:= all_cut_select_head p (flatten_term R1.2) (flatten_mode s.[kp]) fset0 H.
-    by rewrite S/= => /andP[->/all_all_but_last->]; destruct rs'.
-  Qed.
-End mut_excl.
+Lemma all_cut_mut_excl p: good_modes p.(sig) -> all_cut p -> mut_excl u p.
+Proof.
+  rewrite/all_cut/mut_excl push/= => ->/=.
+  case: p => /= + s.
+  elim => //= [[hd bo]] rs/= IH; rewrite !push/=.
+  move=> /andP[HBO] H; rewrite IH// andbT.
+  rewrite/fresh_rule !push/=/mut_excl_head/=.
+  case tm: get_tm_hd => //=[p]; case: fndP => //= kp.
+  (* rewrite push. *)
+  case: ifP => // ds.
+  set R1 := lang.rename _ _ _.
+  case S: select_head => //=[r' rs'].
+  rewrite has_cut_seq_fresh HBO/=.
+  set X := lang.rename (fresh_rules fset0 rs).1 hd empty.
+  have:= all_cut_select_head p (flatten_term R1.2) (flatten_mode s.[kp]) fset0 H.
+  by rewrite S/= => /andP[->/all_all_but_last->]; destruct rs'.
+Qed.
 
 
