theories/unif.v
@@ -11,10 +11,6 @@ Require Import Recdef.
 Require Import Stdlib.Structures.OrdersEx.
 Require Import Stdlib.Wellfounded.Lexicographic_Product .
 
-
-(* Variable u: Unif. *)
-(* Notation matching := (matching u). *)
-(* Notation unify := (unify u). *)
 Notation vars := vars_tm.
 
 Definition compare_var '(IV v1) '(IV v2) := 
@@ -55,7 +51,7 @@ Definition count_varsL k l := sumL (map (map_prod1 addn (count_vars k)) l).
 
 Definition varsL l : fvS := varsU (map (map_prod1 fsetU vars_tm) l).
 
-Definition nvar l := #|` [fset x in (varsL l) | count_varsL x l > 1]|.
+Definition nvar l := #|` varsL l |.
 
 Lemma varsL_cons x xs: varsL (x :: xs) = map_prod1 fsetU vars_tm x `|` varsL xs.
 Proof. by []. Qed.
@@ -71,16 +67,14 @@ Proof. by rewrite/count_varsL//. Qed.
 Lemma nvar_comm x1 x2 xs: nvar ((x1,x2) :: xs) = nvar ((x2, x1) :: xs).
 Proof.
   rewrite /nvar; f_equal; apply/eqP/fset_eqP => i.
-  rewrite 2!inE/= 3![RHS]inE/=; f_equal.
-    by rewrite !varsL_cons map_prod1_comm//; apply/fsetUC.
-  rewrite !count_varsL_cons map_prod1_comm//; apply/addnC.
+  rewrite !varsL_cons map_prod1_comm//; apply/fsetUC.
+  (* rewrite !count_varsL_cons map_prod1_comm//; apply/addnC. *)
 Qed.
 
 Lemma nvar_sub h l : nvar l <= nvar (h :: l).
 Proof.
   apply/fsubset_leq_card/fsubsetP.
-  move=> x; rewrite 2!inE/= 2!inE/= => /andP[H1 H2].
-  rewrite varsL_cons inE H1 orbT count_varsL_cons; lia.
+  by move=> x; rewrite !varsL_cons !inE => ->; rewrite orbT.
 Qed.
 
 Lemma nvar_app f1 a1 f2 a2 tl: 
@@ -88,9 +82,8 @@ Lemma nvar_app f1 a1 f2 a2 tl:
 Proof.
   rewrite/nvar/count_varsL/=/map_prod1/=.
   f_equal; apply/eqP/fset_eqP => x.
-  rewrite 2!inE/= 3![RHS]inE/=; f_equal.
-    rewrite !varsL_cons /map_prod1/= !inE; lia.
-  lia.
+  rewrite !varsL_cons /map_prod1/= !inE.
+  repeat case: (_ \in _) => //.
 Qed.
 
 Fixpoint app_nb t :=
@@ -100,13 +93,29 @@ Fixpoint app_nb t :=
   | Tm_D _ | Tm_P _ => 1
   end.
 
-From Coq Require Import Wellfounded Inverse_Image.
-
 Definition nlhs (l:seqT) := sumL (map app_nb (map fst l)).
 
 Definition neqn (l:seqT) := size l.
 
 Definition measure l := (nvar l, nlhs l, neqn l).
+
+Lemma derefkv_in v t k:
+  v \in vars (derefkv v t k) -> (v \in vars t).
+Proof.
+  elim: k => //=[v'|f Hf a Ha]; last by rewrite inE => /orP[].
+  rewrite/derefkv deref_V fnd_set.
+  case: eqP; rewrite//not_fnd//=; rewrite inE; case: eqP; congruence.
+Qed.
+
+Lemma derefkv_in_ x v t k:
+  x \in vars (derefkv v t k) -> (x \in vars_tm t) || (x \in vars_tm k).
+Proof.
+  elim: k => //=[v'|f Hf a Ha]; last by rewrite !inE => /orP[/Hf|/Ha]/orP[]->; rewrite// !orbT.
+  rewrite/derefkv deref_V fnd_set !inE; case: eqP => [->->//|].
+  by rewrite not_fnd//= inE => H/eqP<-; rewrite eqxx orbT.
+Qed.
+
+From Coq Require Import Wellfounded Inverse_Image.
 
 Definition lex_prod3 (T1 T2: Type) (F: T1 -> T1 -> Prop) (G : T2 -> T2 -> Prop) (x y: T1 * T2) := 
   Relation_Operators.lexprod T1 (fun _ => T2) F (fun _ => G) (existT _ x.1 x.2) (existT _ y.1 y.2).
@@ -133,96 +142,6 @@ Definition lex_seqT (t1 t2: seqT) := lex_prod1 (measure t1) (measure t2).
 Lemma wf_lex_seqT : well_founded lex_seqT.
 Proof. apply/wf_inverse_image/wf_lex_prod1. Qed.
 
-Fixpoint derefkv k v (tm:Tm) :=
-  match tm with
-  | Tm_V k' => if k == k' then v else tm
-  | Tm_P _ | Tm_D _ => tm
-  | Tm_App h ag => Tm_App (derefkv k v h) (derefkv k v ag)
-  end.
-
-Lemma derefvk_in k v l t: k <> v ->
-  k \in vars (derefkv v l t) -> (k \in vars_tm l) || (k \in vars_tm t).
-Proof.
-  move=> H; elim: t => //=[v'|f Hf a Ha]; rewrite !inE.
-    by case: eqP => //=H1; subst; rewrite?inE => ->; rewrite//orbT.
-  by move=> /orP[/Hf|/Ha]/orP[]->//; rewrite !orbT.
-Qed.
-
-Lemma derefvk_in_varsL k v t2 tl:
-  k <> v ->
-  k \in [eta mem_seq (varsL [seq map_prod (derefkv v t2) i | i <- tl])] ->
-  (k \in vars t2) || (k \in varsL tl).
-Proof.
-  move=>H; elim: tl t2 => [|[t1 t2 tl IH]] l.
-    by rewrite inE.
-  rewrite /= !varsL_cons inE => /orP[|/IH]; last first.
-    by rewrite !inE => /orP[] ->//; rewrite !orbT.
-  by rewrite /map_prod1/= !inE => /orP[]/derefvk_in/orP[] => //->; rewrite//!orbT.
-Qed.
-
-(* Lemma count_vars_derefvk_sub :
-  count_vars k (derefkv v t t1) + count_vars k (derefkv v t t2) <=
-    count_vars k t + count_vars k t1.
-
-Lemma count_varsL_derefvk_sub v k t tl:
-  count_varsL k [seq map_prod (derefkv v t) i | i <- tl] <=
-    (v == k) + count_vars k t + count_varsL k tl.
-Proof.
-  elim: tl => -//=[t1 t2] L IH.
-  rewrite !count_varsL_cons /map_prod1/=.
-  rewrite 
-    rewrite /count_varsL//=.
-Admitted. *)
-
-Lemma deref_vk_not_in v t q: v \notin vars t -> v \notin vars (derefkv v t q).
-Proof.
-  move=> vt; elim: q => //=[v'|f Hf a Ha].
-    by case: eqP => //; rewrite inE; case: eqP.
-  by rewrite inE (negbTE Hf)//.
-Qed.
-
-Lemma deref_vkL_not_in v t tl: v \notin vars t ->
-  v \notin [eta mem_seq (varsL [seq map_prod (derefkv v t) i | i <- tl])].
-Proof.
-  move=> vt; elim: tl => //-[t1 t2 l IH]; rewrite /=varsL_cons !inE.
-  by rewrite (negbTE IH) orbF/= negb_or !deref_vk_not_in.
-Qed.
-
-(* Lemma count_varsL_derefvk_not_in:
-
-  count_varsL k [seq map_prod (derefkv v t) i | i <- tl] = count_varsL k tl. *)
-
-Lemma derefvk_sub v t tl:
-  v \notin vars_tm t ->
-  nvar [seq map_prod (derefkv v t) i | i <- tl] < nvar ((Tm_V v, t) :: tl).
-Proof.
-  (* rewrite /nvar => vt; apply/fproper_ltn_card; rewrite fproperE => //=.
-  apply/andP; split.
-    apply/fsubsetP => k; rewrite 2!inE/= 2!inE/=.
-    move=> /andP[H1 H2].
-    rewrite varsL_cons/= inE count_varsL_cons /map_prod1 /=!inE.
-    apply/andP; split.
-      by case: eqP => //= kv; apply/derefvk_in_varsL/H1.
-    case: eqP => ?; subst => /=.
-      by rewrite (negbTE (deref_vkL_not_in tl vt)) in H1.
-    
-    
-    
-
-    by apply/leq_trans/count_varsL_derefvk_sub.
-    have:= count_varsL_derefvk_sub v k t tl.
-    lia.
-    
-    case: eqP => //=.
-    rewrite /map_prod1.
-
-
-    f_equal.
-    rewrite 
-    Search (_ `<` _). *)
-
-Admitted.
-
 Lemma b1 t1 t2 tl:
   (t1 == t2) = true -> lex_seqT tl ((t1, t2) :: tl).
 Proof.
@@ -248,6 +167,24 @@ Proof. rewrite/lex_seqT/measure/=nvar_comm; by constructor 1; constructor 2 => /
 Lemma b3 v d tl: lex_seqT ((Tm_V v, Tm_D d) :: tl) ((Tm_D d, Tm_V v) :: tl).
 Proof. rewrite/lex_seqT/measure/=nvar_comm; by constructor 1; constructor 2 => //=. Qed.
 
+Lemma nvar_cons x xs: nvar (x :: xs) = #|` map_prod1 fsetU vars_tm x `|` varsL xs |.
+Proof. by []. Qed.
+
+Lemma nvar_derefkv' v t tl:
+  nvar [seq map_prod (derefkv v t) i | i <- tl] <=
+    #|` (vars_tm t `|` varsL tl) `\` if v \in vars_tm t then fset0 else [fset v] |.
+Proof.
+  apply/fsubset_leq_card/fsubsetP => k; rewrite !inE.
+  elim: tl => //=x xs IH; rewrite !varsL_cons; rewrite !inE.
+  rewrite/map_prod/=.
+  move=> /orP[|/IH/andP[->/orP[]->]//]; last by rewrite !orbT.
+  case: (boolP (v \in vars_tm t)) => vt2 /=.
+    by move=> /orP[]/derefkv_in_/orP[]->; rewrite//!orbT.
+  rewrite inE; case: eqP => //=kv; subst.
+    by move=> /orP[]/derefkv_in; rewrite (negbTE vt2).
+  by move=> /orP[]/derefkv_in_/orP[]->//; rewrite !orbT.
+Qed.
+
 Lemma b4 v t2 tl:
   (v \in vars t2) = false ->
   lex_seqT [seq map_prod (derefkv v t2) i | i <- tl]
@@ -255,7 +192,11 @@ Lemma b4 v t2 tl:
 Proof.
   rewrite/lex_seqT/measure/=.
   do 2 constructor 1 => /=.
-  by apply/leP/derefvk_sub; rewrite H.
+  rewrite nvar_cons /map_prod1/=.
+  apply/leP/leq_ltn_trans.
+    apply/nvar_derefkv'.
+  rewrite H (cardfsD1 v (v|` _ `|` _)) !inE eqxx add1n.
+  by rewrite !fsetDUl fsetDv fset0U.
 Qed.
 
 Lemma b5 f1 f2 v tl: lex_seqT ((Tm_V v, Tm_App f1 f2) :: tl)
@@ -287,31 +228,27 @@ Proof. rewrite/lex_seqT measure_commV//. Qed.
 
 Opaque measure.
 
-Function montanari is_matching (l: seqT) {wf lex_seqT l} : option Sigma :=
+Function montanari s is_matching (l: seqT) {wf lex_seqT l} : option Sigma :=
   match l with
-  | [::] => Some fmap0
+  | [::] => Some s
   | (t1, t2) :: tl => 
-    if t1 == t2 then montanari is_matching tl
+    if t1 == t2 then montanari s is_matching tl
     else
       match t1, t2 with
-      | Tm_App f1 a1, Tm_App f2 a2 => montanari is_matching ((f1, f2) :: (a1, a2) :: tl)
-      (* | Tm_V v, Tm_V v' =>
-        let: (v, v') := compare_var v v' in
-        let res := montanari is_matching (map (map_prod (derefkv v (Tm_V v'))) tl) in
-          omap (fun x => x.[v <- Tm_V v']) res *)
+      | Tm_App f1 a1, Tm_App f2 a2 => montanari s is_matching ((f1, f2) :: (a1, a2) :: tl)
       | Tm_V v, _ =>
         if (v \in vars_tm t2)  then None
         else 
-          let res := montanari is_matching (map (map_prod (derefkv v t2)) tl) in
-          omap (fun x => x.[v <- t2]) res
-      | _, Tm_V v => if is_matching then None else montanari is_matching ((t2, t1) :: tl)
+          let s := [fmap x : domf s => derefkv v t2 s.[valP x]].[v <- t2] in
+          montanari s is_matching (map (map_prod (derefkv v t2)) tl)
+      | _, Tm_V v => if is_matching then None else montanari s is_matching ((t2, t1) :: tl)
       | _, _ => None
       end
   end.
 Proof.
-  - move=> v l p tl t1 t2 ??; subst; apply: b1.
-  - move=> m l p tl t1 t2 p' ? v ??? /eqP// _ ?; subst; apply/b2.
-  - move=> m l p tl t1 t2 d ? v ??? /eqP// _ ?; subst; apply/b3.
+  - move=> s b l p tl t1 t2 ??; subst; apply: b1.
+  - move=> s m l p tl t1 t2 p' ? v ??? /eqP// _ ?; subst; apply/b2.
+  - move=> s m l p tl t1 t2 d ? v ??? /eqP// _ ?; subst; apply/b3.
   (* - by move=> _ l p t t1 t2 v ? q ??? _ _; subst; apply/b4. *)
   (* - by move=> _ l p t t1 t2 v ? q ??? _ _; subst; apply/b4. *)
   (* - move=> _ l p tl t1 t2 v ? v' ???; case: eqP => // H _ v1 v2; subst.
@@ -320,15 +257,30 @@ Proof.
       by apply/b4; rewrite !inE; case: eqP; congruence.
     apply: lex_seqT_commV.
     by apply/b4; rewrite !inE; case: eqP; congruence. *)
-  - move=> _ l p t t1 t2 v ????; subst; apply/b4.
-  - move=> m l p tl t1 t2 f1 f2 ? v ??? /eqP H ?; subst; apply/b5.
-  - move=> _ l p tl t1 t2 f1 a1 ? f2 a2 ??? /eqP H; subst; apply/b6.
+  - move=> s _ l p t t1 t2 v ????; subst; apply/b4.
+  - move=> s m l p tl t1 t2 f1 f2 ? v ??? /eqP H ?; subst; apply/b5.
+  - move=> s _ l p tl t1 t2 f1 a1 ? f2 a2 ??? /eqP H; subst; apply/b6.
   - apply/wf_lex_seqT.
 Defined.
 
-Definition montanari_pair b t1 t2 := montanari b [::(t1,t2)].
+Ltac montanari_ind s b l :=
+  pattern s, b, l, (montanari s b l);
+  eapply montanari_ind;
+  [
+    have EMPTY := tt; move=> {}s {}b ?? | 
+    have EQ_HD := tt; move=> {}s {}b ? t1 t {}l ? /eqP ? IH| 
+    have APP   := tt; move=> {}s {}b ??? {}l ? []// EQ _ f1 a1 ? f2 a2 ? IH | 
+    have OC_CH := tt; move=> {}s {}b ??? {}l ? []// EQ _ v ? t ? vt | 
+    have U_DER := tt; move=> {}s /={}b ??? {}l ? []// EQ _ v ? t ? []// /negbT vt _ IH| 
+    have MATCH := tt; move=> {}s {}b ??? {}l ? []// EQ _ t ? v ? NV M|
+    have SWAP  := tt; move=> {}s {}b ??? {}l ? []// EQ _ t ? v ? NV []// ? _ IH | 
+    have FAIL  := tt; move=> {}s {}b ??? {}l ? []// EQ _ t1 ? t2 ? H
+  ]; subst.
 
-Goal montanari_pair false (Tm_D (ID 1)) (Tm_V (IV 1)) =
+
+Definition montanari_pair s b t1 t2 := montanari s b [::(t1,t2)].
+
+(* Goal montanari_pair s false (Tm_D (ID 1)) (Tm_V (IV 1)) =
    Some ctx.empty.[IV 1 <- Tm_D (ID 1)].
 Proof. by rewrite /montanari_pair !montanari_equation/=. Qed.
 
@@ -336,15 +288,102 @@ Goal ~ montanari_pair true (Tm_D (ID 1)) (Tm_V (IV 1)).
 Proof. by rewrite /montanari_pair !montanari_equation/=. Qed.
 
 Goal forall b, montanari_pair b (Tm_V (IV 1)) (Tm_D (ID 1)).
-Proof. by move=> b; rewrite/montanari_pair !montanari_equation/=. Qed.
+Proof. by move=> b; rewrite/montanari_pair !montanari_equation/=. Qed. *)
 
 Definition add_ (s:Sigma) r := omap (fun x => x + s) r.
 
-Definition montanari_deref b t1 t2 s := 
-  add_ s (montanari_pair b (deref s t1) (deref s t2)).
+Definition montanari_deref b t1 t2 s := montanari_pair s b (deref s t1) (deref s t2).
 
 Definition matching := montanari_deref true.
 Definition unify := montanari_deref false.
+
+Lemma acyclic_deref v s (vP: v \in domf s):
+  acyclic_sigma s -> v \notin vars_tm (s [` vP]).
+Proof.
+  move=> /fdisjointP/(_ _ vP).
+  apply/contra/fsubsetP/codom_vars_sub_vt.
+Qed.
+
+Lemma acyclic_deref' v s (vP: v \in domf s):
+  acyclic_sigma s -> [disjoint domf s & vars_tm (s [` vP])].
+Proof. by move=> A; apply/fdisjointWr/A/codom_vars_sub_vt. Qed.
+
+(* Lemma deref2 s e t:  *)
+  (* acyclic_sigma (s + e) -> deref s (deref (s + e) t) = deref (s + e) t. *)
+(* Proof. *)
+
+Lemma codom_vars_derefkv s v t:
+  codom_vars  [fmap x : domf s => derefkv v t s.[valP x]] `<=` codom_vars s `|` vars_tm t.
+Proof.
+  rewrite/derefkv.
+  apply/fsubsetP => x/varUP[fv[/mapP[t' /codomP[[z zP ?] ?]xfv]]]; subst.
+  rewrite ffunE valPE in xfv.
+  have:= fsubsetP (vars_tm_deref_sub _ _) _ xfv.
+  rewrite inE codom_vars_set empty_rem inE codom_vars0 !inE/=.
+  move=> /orP[->|]; first by rewrite orbT.
+  move=> H; apply/orP; left; apply/fsubsetP/H/codom_vars_sub_vt.
+Qed.
+
+Lemma acyclic_sigma_derefkv s t v:
+  v \notin vars_tm t -> [disjoint domf s & vars t] ->
+  acyclic_sigma s -> acyclic_sigma [fmap x => derefkv v t s.[valP x]].
+Proof.
+  move=> vt; rewrite /acyclic_sigma/derefkv => df D/=.
+  apply: fdisjointWr.
+    apply: codom_vars_derefkv.
+  by rewrite fdisjointXU D.
+Qed.
+
+
+Lemma acyclic_sigma_derefkv_set s t v:
+  v \notin vars_tm t -> [disjoint domf s & vars t] ->
+  acyclic_sigma s ->
+  acyclic_sigma [fmap x => derefkv v t s.[valP x]].[v <- t].
+Proof.
+  rewrite acyclic_sigma_set => vt D A.
+  have:= acyclic_sigma_derefkv vt D A.
+  move=> /acyclic_sigma_rem->; rewrite vt D andbT !andTb.
+  move: vt; apply/contra.
+  move=> /varUP[w [/mapP[tm + ?]vw]]; subst.
+  move=> /codomP[[x xP] ?]; subst.
+  move: (xP); rewrite domf_rem/= !inE => /andP[xv xs].
+  move: vw.
+  have -> : [fmap x0 => derefkv v t s.[valP x0]].[~ v] [` xP] = [fmap x0 => derefkv v t s.[valP x0]] [` xs].
+    by apply/add_some; rewrite -!in_fnd fnd_rem1 xv.
+  by rewrite ffunE valPE => /derefkv_in.
+Qed.
+
+Lemma montanari_acyclic_aux l s b s':
+  [disjoint domf s & varsU (map (map_prod1 fsetU vars_tm) l)] ->
+  acyclic_sigma s ->
+    montanari s b l = Some s' -> acyclic_sigma s'.
+Proof.
+  move: s'; montanari_ind s b l => s'/=.
+  - by move=> _ A [<-].
+  - by rewrite /map_prod1/= !fdisjointXU => /andP[/andP[dt _]]; apply: IH.
+  - move=> H; apply: IH; move: H; rewrite/map_prod1/= !fsetUA// !fdisjointXU -!andbA.
+    by move=> /and5P[->->->->->].
+  - rewrite /map_prod1 !fdisjointXU/= -!andbA => /and3P[H1 H2 H3] A M.
+    apply: IH (acyclic_sigma_derefkv_set vt _ A) M => //.
+    rewrite/map_prod1 fdisjointUX fdisjoint1X.
+    apply/andP; split.
+      move : vt; apply/contra.
+      move=> /varUP[x[/mapP[tx /mapP[t'] H] ??]]; subst.
+      by rewrite !inE/= => /orP[]/derefkv_in.
+    apply: @fdisjointWr (vars t `|` varsU [seq vars x.1 `|` vars x.2 | x <- l]) _ _ _; last first.
+      by rewrite fdisjointXU H2.
+    apply/fsubsetP => x/varUP[fv[/mapP[tx]/mapP[t' L] ??]]; subst.
+    rewrite !inE/=.
+    by case (boolP (_ \in vars_tm t)) => //= xt/orP[]/derefkv_in_; rewrite (negbTE xt)/= => H;
+    apply/varUP; eexists (vars_tm t'.1 `|` vars_tm t'.2); rewrite inE H ?orbT; split => //;
+    apply/mapP; eexists => //=; auto.
+  - rewrite/map_prod1/= !fdisjointXU -!andbA => /and3P[T H1 D]; apply: IH.
+    by rewrite/map_prod1/= !fdisjointXU H1 T.
+Qed.
+
+Lemma montanari_acyclic b t1 t2 s s':
+  acyclic_sigma s -> montanari_deref b t1 t2 s = Some s' -> acyclic_sigma s'.
+Proof. by move=> A M; apply: montanari_acyclic_aux M; rewrite//=fsetU0/map_prod1/= fdisjointXU !acyclic_deref_disjoint//. Qed.
 
 Lemma omap_catf0 t: omap [eta catf empty] t = t.
 Proof. by case: t => //=?; rewrite cat0f. Qed.
@@ -352,86 +391,290 @@ Proof. by case: t => //=?; rewrite cat0f. Qed.
 Lemma omap_catf_refl (t:Sigma): omap [eta catf t] (Some t) = Some t.
 Proof. by rewrite/=; f_equal; apply/fmapP => k; rewrite fnd_cat if_same. Qed.
 
-Lemma unify_V_empty v t: v \notin vars_tm t -> 
-  unify (Tm_V v) t empty = Some empty.[v <- t].
+Lemma montanari_varl s b v t: v \notin vars_tm t -> 
+  montanari_pair s b (Tm_V v) t = Some [fmap x => derefkv v t s.[valP x]].[v <- t].
 Proof.
-  rewrite/unify/montanari_deref/montanari_pair montanari_equation/= !deref_empty.
-  case: eqP => [<-|vtd vt]; first by rewrite !inE eqxx.
-  by rewrite (negbTE vt) montanari_equation/= catf0.
-  (* rewrite /unify_var/compare_var. !montanari_equation/= (negbTE vt) /add_/= omap_catf0.
-  case: t vtd vt => //= x xs; rewrite inE => H; rewrite !push/=. *)
+  move=> H; rewrite /montanari_pair montanari_equation/= (negbTE H).
+  rewrite 2!montanari_equation/=; case: eqP => //?; subst.
+  by rewrite inE eqxx in H.
 Qed.
 
-Lemma unifier_help_refl b t: montanari_pair b t t = Some fmap0.
+Lemma montanari_var0l b v t: v \notin vars_tm t -> 
+  montanari_pair empty b (Tm_V v) t = Some empty.[v <- t].
+Proof.
+  move=> H; have:= montanari_varl empty b H => ->.
+  by f_equal; apply/fmapP => k; rewrite !fnd_set !not_fnd//.
+Qed.
+
+Lemma unify_V_0l v t: v \notin vars_tm t -> 
+  unify (Tm_V v) t empty = Some empty.[v <- t].
+Proof. by rewrite/unify/montanari_deref !deref_empty => H; apply: montanari_var0l. Qed.
+
+Definition is_var t := match t with Tm_V _ => true | _ => false end.
+
+Lemma unify_V_0r v t: v \notin vars_tm t -> ~~ is_var t ->
+  unify t (Tm_V v) empty = Some empty.[v <- t].
+Proof.
+  rewrite/unify/montanari_deref/montanari_pair.
+  rewrite !deref_empty montanari_equation.
+  case: eqP => [->|]; first by rewrite inE eqxx.
+  move=> H1 vt => H.
+  suffices : montanari empty false [:: (Tm_V v, t)] = Some empty.[v <- t].
+    move=> ->; destruct t => //.
+  by apply/montanari_var0l.
+Qed.
+
+Lemma unifier_help_refl s b t: montanari_pair s b t t = Some s.
 Proof. rewrite/montanari_pair montanari_equation eqxx montanari_equation//. Qed.
 
 Lemma unifier_help_refl1 b t s: montanari_deref b t t s = Some s.
-Proof. by rewrite /montanari_deref unifier_help_refl/= cat0f. Qed.
+Proof. by rewrite /montanari_deref unifier_help_refl. Qed.
 
 Lemma unify_refl t s: unify t t s = Some s.
 Proof. apply/unifier_help_refl1. Qed.
 
-Ltac montanari_ind b l :=
-  pattern b, l, (montanari b l);
-  eapply montanari_ind;
-  [
-    move=> {}b ?? | 
-    move=> {}b ? t1 t2 {}l ? EQ IH| 
-    move=> {}b ??? {}l ? []// EQ _ f1 a1 ? f2 a2 ? IH | 
-    move=> {}b ??? {}l ? []// EQ _ v ? t ? vt | 
-    move=> /={}b ??? {}l ? []// EQ _ v ? t ? []// vt _ IH| 
-    move=> {}b ??? {}l ? []// EQ _ t ? v ? NV M|
-    move=> {}b ??? {}l ? []// EQ _ t ? v ? NV []// ? _ IH | 
-    move=> {}b ??? {}l ? []// EQ _ t1 ? t2 ? H
-  ]; subst.
-
-Lemma montanari_cons_ground b t1 t2 l:
-  t1 != t2 -> ground t1 -> ground t2 -> ~~ montanari b ((t1, t2) :: l).
+Lemma montanari_match_unif l s s':
+  montanari s true l = Some s' -> montanari s false l = Some s'.
 Proof.
-  elim: t1 t2 l => [p|d|v|f Hf a Ha] + l.
-    move=> [p'|d'|v'|f' a']//; rewrite montanari_equation//?ground_V// => /negbTE->//.
-    move=> [p'|d'|v'|f' a']//; rewrite montanari_equation//?ground_V// => /negbTE->//.
-    by move=> ?; rewrite ground_V.
-  move=> t2; rewrite montanari_equation => /[dup]+/negbTE->.
-  case: t2 => [p'|d'|v'|f' a']//; rewrite !(ground_app,ground_V)//.
-  move=> H /andP[gf ga] /andP[gf' ga'].
-  case: (boolP (f == f')) => [/eqP?|?]; last by apply: Hf.
-  subst; rewrite montanari_equation eqxx Ha//.
-  by apply/eqP => ?; subst; rewrite eqxx in H.
+  move: false => b; move: s'.
+  montanari_ind s b l => s'.
+  - by rewrite montanari_equation.
+  - by rewrite montanari_equation eqxx; auto.
+  - by rewrite montanari_equation EQ; auto.
+  - by rewrite montanari_equation EQ vt.
+  - by rewrite montanari_equation EQ (negbTE vt); apply: IH.
+  - by rewrite montanari_equation EQ; destruct t.
+  - by rewrite montanari_equation EQ; destruct t.
+  - by rewrite montanari_equation EQ; destruct t1, t2.
 Qed.
 
-Lemma unify_help_ground b t1 t2: 
-  ground t1 -> ground t2 -> (t1 == t2) = (montanari_pair b t1 t2).
+Definition disjoint_L (s:Sigma) l:=
+  [disjoint domf s & varsU (map (map_prod1 fsetU vars_tm) l)].
+
+Lemma disjoint_L_cons s x xs:
+  disjoint_L s (x :: xs) =
+    [&&fdisjoint (domf s) (vars_tm x.1), fdisjoint (domf s) (vars_tm x.2) 
+    & disjoint_L s xs].
+Proof. by case: x => [t1 t2]; rewrite/disjoint_L/= !fdisjointXU andbA. Qed.
+
+Lemma disjoint_L_set s v t l: v \notin vars t ->
+  [disjoint domf s & vars t] -> disjoint_L s l ->
+  disjoint_L [fmap x => derefkv v t s.[valP x]].[v <- t]
+    [seq map_prod (derefkv v t) i | i <- l].
 Proof.
-  rewrite/montanari_pair.
-  case: eqP => //[->|]; first by rewrite 2!montanari_equation eqxx.
-  by move=> /eqP H1 G1 G2; apply/esym/negbTE/montanari_cons_ground.
+  rewrite/disjoint_L dom_setf/= => vt D H.
+  apply/fdisjointP => x xP.
+  move: vt; apply/contra => /varUP[q[/mapP[?/mapP[t1 H1]?]?]H2]; subst.
+  move: xP; rewrite !inE; case: eqP => /=[? _|xv xs]; subst.
+    by rewrite/map_prod1 inE/= in H2; move/orP: H2 => []/derefkv_in.
+  move: H2; rewrite/map_prod1/=inE => /orP[] Hx.
+    have := derefkv_in_ Hx => /orP[] Hy.
+      by have:= fdisjointP D _ xs; rewrite Hy.
+    have:= fdisjointP H _ xs.
+    move=> /varUP[]; exists (vars t1.1 `|` vars t1.2); split; last by rewrite inE Hy.
+    by apply/mapP; rewrite /map_prod1; eexists => //.
+  have := derefkv_in_ Hx => /orP[] Hy.
+    by have:= fdisjointP D _ xs; rewrite Hy.
+  have:= fdisjointP H _ xs.
+  move=> /varUP[]; exists (vars t1.1 `|` vars t1.2); split; last by rewrite inE Hy orbT.
+  by apply/mapP; rewrite /map_prod1; eexists => //.
 Qed.
 
-(* Lemma unify_help_groundx b n t1 t2 s: 
-  ground t1 -> ground t2 -> t1 <> t2 -> unifier_help b n t1 t2 s = None.
+Lemma montanari_ext b l s s': montanari s b l = Some s' -> domf s `<=` domf s'.
 Proof.
-  move=> G1 G2 H; have:= unify_help_ground b n s G1 G2.
-  by case: eqP => //;rewrite/unify; case: unifier_help.
+  move: s'; montanari_ind s b l => s'.
+  - move=> [<-]//.
+  - by apply: IH.
+  - move=> /IH/fsubsetP => H; apply/fsubsetP => x xs.
+    by have:= H x; rewrite inE xs orbT => /(_ isT).
 Qed.
 
-Lemma unify_help1_groundx b t1 t2 s: 
-  ground t1 -> ground t2 -> t1 <> t2 -> unifier_help1 b t1 t2 s = None.
+
+Definition mp (o n: Sigma) :=
+  [forall x : domf o, Some (deref n o.[valP x]) == n.[? val x]].
+
+Lemma derefxx o n t:
+  mp o n -> deref n (deref o t) = deref n t.
 Proof.
-  move=> G1 G2 H; have:= unify_help_ground b (size_tm t1 + size_tm t2) s G1 G2.
-  rewrite/unifier_help1; case: eqP => // _; case: unifier_help => //.
+  move=> A; elim: t => //[v|/=f->a->//].
+  rewrite !deref_V; case: fndP => //=vo.
+  have:= forallP A [`vo]; rewrite valPE/= => /eqP<-//.
 Qed.
 
-Lemma unify_help2_groundx b t1 t2 s: 
-  ground t1 -> ground t2 -> t1 <> t2 -> unifier_help2 b t1 t2 s = None.
-Proof.
-  move=> G1 G2 H; have:= unify_help1_groundx b s G1 G2 H.
-  by rewrite/unifier_help2 !ground_deref//.
-Qed. *)
+Lemma mp_id s: acyclic_sigma s -> mp s s.
+Proof. 
+  move=> A; apply/forallP => -[x xs]/=; rewrite valPE/= in_fnd not_in_deref//.
+  by apply/fdisjointWr/A/codom_vars_sub_vt.
+Qed.
 
-(* Lemma unify_diff_ground t1 t2 s: 
-  ground t1 -> ground t2 -> t1 <> t2 -> unify t1 t2 s = None.
-Proof. by apply/unify_help2_groundx. Qed. *)
+Lemma mp_set s s' v t: v \notin vars_tm t -> v \notin domf s ->
+  [disjoint domf s & vars t] -> mp s.[v <- t] s' -> mp s s'.
+Proof.
+  move=> vt vs D H; apply/forallP => -[/= x xs]; rewrite valPE.
+  move /forallP: H.
+  have H: x \in (domf s.[v <- t]) by rewrite !inE/= xs orbT.
+  move=> /(_ [`H]); rewrite ffunE valPE/= => /eqP.
+  rewrite in_fnd/=; case: eqP => //=; last move=> _ <-//.
+  move=> ?; subst; case: fndP => //= s'v[]; clear H.
+  by rewrite xs in vs.
+Qed.
+
+Lemma mp_cat x sub s' t:
+  mp (x + sub) s' -> deref s' (deref sub t) = deref s' t.
+Proof.
+  move=> H.
+  elim: t => //=[v|f -> a ->//].
+  case: fndP => vsub//=.
+  have vP: v \in domf (x + sub) by rewrite !inE vsub orbT.
+  have:= forallP H [`vP]; rewrite valPE getf_catr/=.
+  case: fndP => //vs'/=/eqP[]//.
+Qed.
+
+Lemma didi x v t s':
+  mp x.[v <- t] s' -> Some (deref s' t) = s'.[? v].
+Proof.
+  move=> H; have H1: v \in v |` domf x by rewrite !inE eqxx.
+  by have:= forallP H [`H1]; rewrite valPE/= ffunE/= eqxx => /eqP.
+Qed.
+
+Lemma mp_derefkv s s' v t: v \notin vars_tm t -> v \notin domf s ->
+  [disjoint domf s & vars t] -> mp [fmap x => derefkv v t s.[valP x]].[v <- t] s' -> mp s s'.
+Proof.
+  move=> vt vs D H; apply/forallP => -[/= x xs]; rewrite valPE.
+  move /forallP: (H).
+  have H1: x \in (domf s.[v <- t]) by rewrite !inE/= xs orbT.
+  move=> /(_ [`H1]); rewrite ffunE valPE/= => /eqP.
+  case: fndP => //xs'; case: eqP => xv; subst; first by rewrite xs in vs.
+  rewrite (@in_fnd _ _ [ffun x0 => _] x)/= ffunE valPE.
+  rewrite derefxx// => [->|]//.
+  apply/forallP => /=; rewrite fsetU0 => -[y yv].
+  rewrite !ffunE/=.
+  move: yv; rewrite inE => /eqP?; subst.
+  rewrite eqxx.
+  apply/eqP/didi/H.
+Qed.
+
+Lemma montanari_mp b l s s': acyclic_sigma s ->
+  disjoint_L s l -> montanari s b l = Some s' -> mp s s'.
+Proof.
+  move: s'; montanari_ind s b l => s' A.
+  - by move=> _ [<-]; apply/mp_id.
+  - by rewrite disjoint_L_cons => /and3P[H1 H2]; apply: IH.
+  - rewrite disjoint_L_cons/= !fdisjointXU -!andbA => /and5P[D1 D2 D3 D4] D.
+    by apply:IH; rewrite //!disjoint_L_cons D1 D2 D3 D4.
+  - rewrite disjoint_L_cons/=fdisjointX1 => /and3P[vs D H] M.
+    have {}IH := IH _ (acyclic_sigma_derefkv_set vt D A) (disjoint_L_set vt D H) M.
+    apply/mp_derefkv/IH => //.
+  - rewrite disjoint_L_cons/= => /and3P[D1 D2 H]; apply: IH => //.
+    by rewrite disjoint_L_cons/= D2 D1.
+Qed.
+
+Lemma montanari_set_deref' b s s' l x sub t: 
+  acyclic_sigma s -> disjoint_L s l -> x + sub = s ->
+  montanari s b l = Some s' -> deref s' (deref sub t) = (deref s' t).
+Proof.
+  move=> A D ? M; subst.
+  have:= montanari_mp A D M.
+  by apply/mp_cat.
+Qed.
+
+Lemma montanari_set_deref v b s s' l (vs : v \in domf s) (vs': v \in domf s'): 
+  acyclic_sigma s -> disjoint_L s l ->
+  montanari s b l = Some s' -> (deref s' s.[vs]) = s'.[vs'].
+Proof.
+  move=> A D M; subst.
+  have:= montanari_mp A D M.
+  replace s'.[vs'] with (deref s' (Tm_V v)); last by rewrite/=in_fnd.
+  replace s.[vs] with (deref s (Tm_V v)); last by rewrite/=in_fnd.
+  rewrite -{1}(@cat0f _ _ s); apply/mp_cat.
+Qed.
+
+Lemma montanariP b l s s': acyclic_sigma s -> disjoint_L s l ->
+  montanari s b l = Some s' -> all (map_prod1 (eq_op) (deref s')) l.
+Proof.
+  move: s'; montanari_ind s b l => s' A.
+  - by [].
+  - by rewrite disjoint_L_cons => /and3P[_ _]; rewrite/map_prod1/=eqxx; apply: IH.
+  - rewrite disjoint_L_cons/= !fdisjointXU -2!andbA /map_prod1.
+    move=> /and5P[D1 D2 D3 D4 D5] M.
+    have:= IH _ A _ M; rewrite /= !disjoint_L_cons/= D1 D2 D3 D4 D5 => /(_ isT).
+    by rewrite /map_prod1/= => /andP[/eqP->/andP[/eqP->]]; rewrite eqxx.
+  - rewrite disjoint_L_cons/= => /and3P[D1 D2 D3] M.
+    have A': acyclic_sigma [fmap x => derefkv v t s.[valP x]].[v <- t].
+      rewrite acyclic_sigma_set vt acyclic_sigma_rem.
+        rewrite !andTb; apply/andP; split => //.
+        have:= vt; apply/contra.
+        move=> /varUP[z[/mapP[?/codomP[[t' t'P] ??]]]]; subst.
+        move: t'P (t'P); rewrite {1}domf_rem !inE => /andP[H1 H2].
+        simpl in H2 => t'P.
+        have -> : [fmap x => derefkv v t s.[valP x]].[~ v] [` t'P] = ([fmap x => derefkv v t s.[valP x]] [` H2]).
+          by apply/add_some; rewrite -!in_fnd !fnd_rem inE (negbTE H1).
+        by rewrite ffunE valPE; apply/derefkv_in.
+      by apply: acyclic_sigma_derefkv => //; rewrite vt.
+    have D : disjoint_L [fmap x => derefkv v t s.[valP x]].[v <- t]
+      [seq map_prod (derefkv v t) i | i <- l].
+      by apply/disjoint_L_set => //; rewrite vt.
+    have {IH} := IH _ A' D M.
+    rewrite {1 2}/map_prod1/= => H.
+    apply/andP; split.
+      rewrite in_fnd.
+        by have:= fsubsetP (montanari_ext M) => /(_ v); rewrite !inE/= eqxx=>->.
+      move=> vs'/=.
+      have:= montanari_set_deref _ _ _ _ M.
+      move=> /(_ _ _ vs').
+      move=> <-//; first by rewrite !inE eqxx.
+      by move=> H1; rewrite ffunE/= eqxx.
+    rewrite all_map in H.
+    apply/allP => xt Ht.
+    have /=:= allP H _ Ht.
+    rewrite/map_prod1.
+    have:= montanari_set_deref' _ _ _ _ M.
+    move=> /(_ [fmap x => derefkv v t s.[valP x]] [fmap].[v <- t] _ A' D).
+    rewrite catf_setr catf0 => /(_ _ erefl) Hq.
+    by rewrite !Hq.
+  - rewrite disjoint_L_cons => /and3P[D1 D2 D3] M.
+    have:= IH _ A _ M; rewrite disjoint_L_cons/= D1 D2 D3 => /(_ isT).
+    by rewrite/map_prod1/= eq_sym => ->.
+Qed.
+
+Lemma montanari_ground s b l:
+  all (map_prod1 andb ground) l -> 
+  montanari s b l = if all (fun '(x, y) => x == y) l then Some s else None.
+Proof.
+  montanari_ind s b l => //=.
+  - by rewrite /map_prod1 eqxx/= => /andP[_/IH].
+  - rewrite/map_prod1/=!ground_app/= -3!andbA => /and5P[g1 g2 g3 g4 g5].
+    rewrite IH//=/map_prod1/=; last by rewrite -!andbA g1 g2 g3 g4.
+    case: eqP => [->|]/=.
+      case: eqP => [->|]; first by rewrite eqxx.
+      case: eqP => ??//; congruence.
+    case: eqP => //; congruence.
+  - by rewrite EQ.
+  - by rewrite/map_prod1 ground_V.
+  - by rewrite/map_prod1/= ground_V andbF.
+  - by rewrite/map_prod1/= ground_V andbF.
+  - by rewrite /=EQ.
+Qed.
+
+Lemma montanari_pair_ground s b t1 t2: 
+  ground t1 -> ground t2 -> montanari_pair s b t1 t2 = if t1 == t2 then Some s else None.
+Proof.
+  move=> G1 G2; have:= @montanari_ground s b [::(t1,t2)].
+  by rewrite /map_prod1/= G1 G2 !andbT => /(_ isT).
+Qed.
+
+Lemma unify_ground s t1 t2: 
+  ground t1 -> ground t2 -> unify t1 t2 s = if t1 == t2 then Some s else None.
+Proof. move=> G1 G2; rewrite/unify/montanari_deref !ground_deref//montanari_pair_ground//. Qed.
+
+Lemma unify_derefl s t1 t2: acyclic_sigma s ->
+  unify t1 t2 s = unify (deref s t1) t2 s.
+Proof. move=> A; rewrite /unify/montanari_deref deref2//. Qed.
+
+Lemma unify_derefr s t1 t2: acyclic_sigma s ->
+  unify t1 t2 s = unify t1 (deref s t2) s.
+Proof. move=> A; rewrite /unify/montanari_deref deref2//. Qed.
+
 
 Lemma isSomeP T x (P : option T) : P = Some x -> P.
 Proof. by move=> ->. Qed.
@@ -442,21 +685,6 @@ Proof. by move=> ->. Qed.
 Lemma isNoneP1 T (P : option T) : ~~ P -> P = None.
 Proof. case: P => //. Qed.
 
-Lemma montanari_match_unif l s:
-  montanari true l = Some s -> montanari false l = Some s.
-Proof.
-  move: false => b; move: s.
-  montanari_ind b l => s.
-  - by rewrite montanari_equation.
-  - by rewrite montanari_equation EQ; auto.
-  - by rewrite montanari_equation EQ; auto.
-  - by rewrite montanari_equation EQ vt.
-  - rewrite montanari_equation EQ vt; case M: montanari => [s'|]//=[?]; subst.
-    rewrite (IH s')//.
-  - by rewrite montanari_equation EQ; destruct t.
-  - by rewrite montanari_equation EQ; destruct t.
-  - by rewrite montanari_equation EQ; destruct t1, t2.
-Qed.
 
 Lemma match_unif t1 t2 s s': matching t1 t2 s = Some s' -> unify t1 t2 s = Some s'.
 Proof.
@@ -474,67 +702,15 @@ Lemma add_eq0 a b: ((addn a b) == 0) = (a == 0) && (b == 0).
 Proof. case: a => //. Qed.
 
 (*SNIPT: unif_trans *)
-Lemma unif_trans t1 t2 t3 s: unify t1 t2 s -> unify t2 t3 s -> unify t1 t3 s.
+(* Lemma unif_trans t1 t2 t3 s: 
+  unify t1 t2 s = Some s' -> unify t2 t3 s' -> unify t1 t3 s.
 (*ENDSNIPT: unif_trans *)
 Proof.
-Admitted.
+Admitted. *)
 
 Lemma eq_app f1 a1 f2 a2:
   (Tm_App f1 a1 == Tm_App f2 a2) = (f1 == f2) && (a1 == a2).
 Proof. do 3 case:eqP => //; congruence. Qed.
-
-Lemma montanariP b l s:
-  montanari b l = Some s -> all (map_prod1 (eq_op) (deref s)) l.
-Proof.
-  move: s; montanari_ind b l => s//=.
-  - by move/eqP: EQ => -> /IH; rewrite/map_prod1/=eqxx.
-  - by move=> /IH/=; rewrite {1 2 4}/map_prod1/= !deref_App eq_app => /and3P[->->].
-  - case M: montanari => [s'|]//=[?]; subst; move: M.
-    move=> /IH H.
-    apply/andP; split.
-      rewrite/map_prod1/=.
-      admit.
-    admit.
-  - move=> /IH/=/andP[+->]; rewrite andbT /map_prod1/= eq_sym//.
-Admitted.
-
-(* Lemma unify_help_ext n t1 t2 s s':
-  montanari_pair false n t1 t2 s = Some s' ->
-    exists e : finMap lang_V__canonical__choice_Choice Tm,
-      [disjoint domf e & domf s] /\ s' = s + e.
-Proof.
-  elim: n t1 t2 s s' => //= [|n IH] t1 t2 s s'.
-    by case: eqP => // H [<-]; exists empty; rewrite catf0 fdisjoint0X.
-  case: eqP => // DE; first by move=> [<-]; exists empty; rewrite catf0 fdisjoint0X.
-  rewrite/unify_var/=.
-  case D1: deref => [p|d|v|f a].
-  - case D2: deref => [p'|d'|v'|f' a']//= [?]; subst; exists [fmap].[v' <- Tm_P p].
-    rewrite catf_setr catf0//= fsetU0 fdisjoint1X; split => //.
-    admit.
-  - case D2: deref => [p'|d'|v'|f' a']//= [?]; subst; exists [fmap].[v' <- Tm_D d].
-    rewrite catf_setr catf0//= fsetU0 fdisjoint1X; split => //.
-    admit.
-  - case: (boolP (_ \in _)) => //.
-    admit.
-  - case D2: deref => [p|d|v|f' a']//.
-      case: (boolP (_ \in _)) => // vd1[<-]; exists [fmap].[v <- Tm_App f a].
-      rewrite catf_setr catf0//= fsetU0 fdisjoint1X; split => //.
-      admit.
-    case Uf: unifier_help => [sx|]//= Ua.
-    have:= IH _ _ _ _ Uf; have:= IH _ _ _ _ Ua.
-    move=> [sy[D ?]][sz[R ?]]; subst.
-    move: D; rewrite domf_cat fdisjointXU => /andP[S T].
-    by exists (sz + sy); rewrite catfA domf_cat fdisjointUX R S.
-Admitted. *)
-
-
-(* Lemma unif_ext t1 t2 s s': unify t1 t2 s = Some s' ->
-  exists e, [disjoint domf e & domf s] /\ s' = s + e.
-Proof.
-  rewrite/unify/unifier_help2/unifier_help1.
-  case U: unifier_help => [sx|]//=[?]; subst.
-  exists sx; split => //.
-Admitted. *)
 
 Inductive swap : seqT -> seqT -> Prop :=
 | swap0 : swap [::] [::]
@@ -543,11 +719,10 @@ Inductive swap : seqT -> seqT -> Prop :=
 
 Lemma swap_map f l1 l2: swap l1 l2 -> swap (map (map_prod f) l1) (map (map_prod f) l2).
 Proof. by (elim => /=; clear) => [|t1 t2 l1 l2 H IH|t1 t2 l1 l2 H IH]; constructor. Qed.
-  
 
-Definition is_var t := match t with Tm_V _ => true | _ => false end.
 
-Lemma montanari_commS b l1 l2 s:
+(* TODO: here *)
+(* Lemma montanari_commS b l1 l2 s:
   b = false -> swap l1 l2 -> montanari b l1 = Some s -> montanari b l2.
 Proof.
   move: l2 s; montanari_ind b l1 => l2 s ?; subst => //.
@@ -585,7 +760,7 @@ Proof.
   admit.
   inversion 1; subst; rewrite montanari_equation ?(eq_sym t2) EQ; 
   destruct t2, t1 => //.
-Admitted.
+Admitted. *)
 
 (* Definition swaps_aux (s : Sigma) :=
   let d := filterf s (fun x => if s.[?x] is Some (Tm_V v) then true else false) in
@@ -612,51 +787,8 @@ Definition is_var t := if t is (Tm_V _) then true else false. *)
  unif sigma A /\ 
  forall tau, unif tau A -> forall s, tau (sigma s) = tau s. *)
 
-(* Axiom phi: Tm -> Tm -> Sigma.
-
-Axiom xx: forall t1 t2 s s', 
-  unify t1 t2 s = Some s' -> deref s' t1 = deref s' (deref (phi t1 t2) t1). *)
-
-(* f X X = f Z Y ====> {X = Z; Z = Y} *)
-(* f Z Y = f X X ====> {Y = X; Z = X} *)
-(* Lemma unif_symP t1 t2 s s':
-  unify t1 t2 s = Some s' -> unify t2 t1 s = Some (swap s s').
-Proof.
-  rewrite/unify/vars_nb addnC.
-  move: (_+_)%nat => n; elim: n t1 t2 s s' => //= [|n IH] t1 t2 s s'.
-    by rewrite/= eq_sym; case: eqP => // D [<-]; rewrite swap_refl.
-  rewrite eq_sym; case: eqP => // DE.
-    by move=> [<-]; rewrite swap_refl.
-  rewrite/unify_var/=; move: DE.
-  case D1: deref => [p|d|v|f a].
-  - case D2: deref => [p'|d'|v'|f' a']//=; move=> DE [<-]; f_equal.
-    admit.
-  - case D2: deref => [p'|d'|v'|f' a']//=; move=> DE [<-]; f_equal.
-    admit.
-  - case: (boolP (_ \in _)) => // H + [<-].
-    case: (boolP (is_var (deref s t1))).
-      case D2: deref => [p'|d'|v'|f' a']//=.
-      rewrite !inE; case: eqP => //?; subst => //.
-      admit.
-    move=> IV Hx.
-    suffices: s.[v <- deref s t1] = (swap s s.[v <- deref s t1]).
-      by move: IV => + <-; case: deref => //.
-    admit.
-  - case D2: deref => [p'|d'|v'|f' a']//=.
-      rewrite !inE; case: (boolP (_ \in _)) => //=vf.
-      case: (boolP (_ \in _)) => //=va _ [<-].
-      admit.
-    move=> H.
-    rewrite-/unify_var.
-    case U1: unifier_help => [sz|]//= U2.
-    have [e[Dx ?]] := unify_help_ext U1; subst.
-    have [e'[Dy ?]] := unify_help_ext U2; subst.
-    have Hf := IH _ _ _ _ U1.
-    have Ha := IH _ _ _ _ U2.
-    rewrite Hf/=.
-Admitted. *)
-
-Lemma unif_sym t1 t2 s: unify t1 t2 s = unify t2 t1 s.
+(* TODO: *)
+(* Lemma unif_sym t1 t2 s: unify t1 t2 s = unify t2 t1 s.
 Proof.
   rewrite/unify/montanari_deref/montanari_pair.
   case M: montanari => //=.
@@ -672,44 +804,29 @@ Proof.
     by rewrite/unify_var !inE eq_sym compare_var_sym.
   rewrite IH.
   case U1: unifier_help => [s'|]//=.
-Qed.
+Qed. *)
 
 (* Lemma unif_sym t1 t2 s: unify t1 t2 s -> unify t2 t1 s.
 Proof. case U: unify => //_; apply/isSomeP. /unif_symP/U. Qed. *)
 
 
-Axiom unif_acyclic: forall t1 t2 s s',
+Lemma unif_acyclic t1 t2 s s':
   acyclic_sigma s -> unify t1 t2 s = Some s' -> acyclic_sigma s'.
+Proof. apply/montanari_acyclic. Qed.
 
-Lemma matching_acyclic: forall t1 t2 s s',
+Lemma matching_acyclic t1 t2 s s':
   acyclic_sigma s -> matching t1 t2 s = Some s' -> acyclic_sigma s'.
-Proof. by move=> > A /match_unif; apply: unif_acyclic. Qed.
+Proof. by apply/montanari_acyclic. Qed.
 
 Axiom matching_subst : forall q t s, 
   [disjoint vars q & domf s] ->
-  (matching q (deref s t) fmap0) <-> (matching q t s).
+  (matching (deref s t) q fmap0) <-> (matching t q s).
 
 Notation "t1 # t2" := [disjoint t1 & t2] (at level 20).
 
-Search deref fdisjoint.
-
-Lemma disjoint_deref1_refl s t:
-  vars t # domf s -> deref1 s t = t.
-Proof.
-  elim: t => //= [v|f Hf a Ha].
-    by rewrite fdisjoint1X => H; rewrite not_fnd.
-  rewrite fdisjointUX => /andP[/Hf-> /Ha->]//.
-Qed.
-
-Lemma disjoint_deref_refl s t:
-  vars t # domf s -> deref s t = t.
-Proof.
-  rewrite/deref; move: #|`_| => n; elim: n t => //= n IH t H.
-  by rewrite disjoint_deref1_refl//IH.
-Qed.
-
+(* TODO: *)
 (*SNIPT: matchdisj *)
-Lemma matching_disj:
+(* Lemma matching_disj:
   forall s s' t1 t2, vars t1 # domf s -> vars t1 # vars t2 ->
                                                                   (*SHOULD BE: e `<=` vars (deref s t2)*)
     matching t1 t2 s = Some s' -> exists e, domf s' = domf s `|` e /\ e `<=` vars t2.
@@ -718,31 +835,53 @@ Proof.
   rewrite/matching/unifier_help2/unifier_help1 => s s' t1 t2.
   case U: unifier_help => //=[sx] V1 V2[?]; subst.
   exists (domf sx); rewrite domf_cat; split => //.
+Admitted. *)
+
+Lemma montanari_monotoneR b s sx l1 l2:
+  all2 (fun x y => (x.2 == y.2) && (deref sx y.1 == x.1)) l1 l2 ->
+  montanari s b l1 -> montanari s b l2.
+Proof.
+  move: l2 => /=; montanari_ind s b l1.
+  - by move=> []//=; rewrite montanari_equation//.
+  - move=> []//=[l r] tl/= /andP[/andP[/eqP?/eqP?] A] M; subst.
+    have:= IH _ A M.
+    admit.
+  - move=> []//=[l r] tl/= /andP[/andP[/eqP?/eqP D] A] M; subst.
+    have:= IH tl _ M.
+    rewrite /=.
+    admit.
+
 Admitted.
 
 (*SNIPT: matchingmono *)
-Axiom matching_monotone: 
-  forall q t s, matching q (deref s t) fmap0 -> matching q t fmap0.
+Lemma matching_monotone q t s:
+  matching (deref s t) q fmap0 -> matching t q fmap0.
 (*ENDSNIPT: matchingmono *)
-
+Proof.
+  rewrite/matching/montanari_deref !deref_empty.
+  rewrite/montanari_pair/=.
+  have HH := @montanari_monotoneR true ctx.empty s .
+  by apply: HH => //=; rewrite !eqxx.
+Qed.
 
 Lemma matching_subst1:
   forall q t s, 
   [disjoint vars q & domf s] ->
-  (matching q t s) -> (matching q (deref s t) fmap0).
-Proof. by move=> > H1 H2; apply/matching_subst. Qed.
+  (matching t q s) -> (matching (deref s t) q fmap0).
+Proof. move=> > H1 H2; apply/matching_subst => //=. Qed.
 
 Lemma matching_subst2:
   forall q t s, 
   [disjoint vars q & domf s] ->
-  (matching q (deref s t) fmap0) -> (matching q t s).
+  (matching (deref s t) q fmap0) -> (matching t q s).
 Proof. by move=> > H1 H2; apply/matching_subst. Qed.
 
 Lemma unif_match a b s:
   unify a b s = None -> matching a b s = None.
 Proof. case m: matching => [s'|]//; rewrite (match_unif m)//. Qed.
 
-Lemma match2_unif : forall q t1 t2 s,
+(* TODO: *)
+(* Lemma match2_unif : forall q t1 t2 s,
   (matching q t1 s) -> (matching q t2 s) -> (unify t1 t2 s).
 Proof.
   move=> q t1 t2 s.
@@ -752,16 +891,14 @@ Proof.
   move=> H1 H2.
   rewrite unif_sym in H2.
   apply/unif_trans/isSomeP/H1/isSomeP/H2.
-Qed.
+Qed. *)
 
 Axiom matching_V: forall s t d,
   vars_sigma s `<=` d -> vars t `<=` d ->
   matching t (Tm_V (fresh d)) s = Some (s.[fresh d <- t]).
 
-Notation "A | B" := (A `|` B) (at level 15).
 Notation injective := (@injectiveb _ V).
 Notation "A ∧ B" := (A && B) (at level 15).
-Notation rename := ren.
 
 (*SNIPT: refresh_for *)
 Definition refresh_for x t := 
@@ -773,50 +910,9 @@ Definition refresh_for x t :=
 Axiom unif_ren: 
   forall x y z w t1 t2,
   refresh_for w t1 -> refresh_for y t2 -> refresh_for z t1 -> refresh_for x t2 ->
-  codomf w # vars (rename y t2) -> codomf z # vars (rename x t2) ->
-  unify (rename w t1) (rename y t2) empty -> unify (rename z t1) (rename x t2) empty.
+  codomf y # vars (ren w t1) -> codomf x # vars (ren z t1) ->
+  unify (ren w t1) (ren y t2) empty -> unify (ren z t1) (ren x t2) empty.
 (*ENDSNIPT: unif_ren *)  
 
 Lemma good_ren_app x f a: refresh_for x (Tm_App f a) = refresh_for x f && refresh_for x a.
 Proof. rewrite/refresh_for/= fsubUset !andbA -!(andbC (injective x)) !andbA andbb !(andbC _ (_ # _)) !andbA andbb//. Qed.
-
-Lemma disjoint_sub {T: choiceType} (s1 s2 s3: {fset T}):
-  [disjoint s1 & s2] ->
-  s3 `<=` s2 -> [disjoint s1 & s3].
-Proof.
-  move=> /eqP H1 D; apply/eqP; move: H1 D.
-  move=> /fsetP I /fsubsetP S; apply/fsetP => x.
-  have:= I x; have:= S x.
-  rewrite !in_fsetI; case: (x \in s1) => //=.
-  by case: (_ \in s3) => //=->//.
-Qed.
-
-Lemma disjointUr {T:choiceType} (A B C: {fset T}): 
-  fdisjoint A (B `|` C) = fdisjoint A B && fdisjoint A C.
-Proof. by rewrite/fdisjoint fsetIUr fsetU_eq0//. Qed.
-
-Lemma disjointUl {T:choiceType} (A B C: {fset T}): 
-  fdisjoint (B `|` C) A = fdisjoint B A && fdisjoint C A.
-Proof. by rewrite fdisjoint_sym disjointUr !(fdisjoint_sym A). Qed.
-
-Lemma deref_disj_id s t: domf s # vars t -> deref s t = t.
-Proof. 
-  elim: t => //=[p|d|v|f Hf a Ha]; rewrite ?(deref_P,deref_D,deref_App)//.
-    rewrite/fdisjoint fsetI1; case: ifP.
-      by move=> _ /eqP/fsetP/(_ v); rewrite !inE eqxx.
-    move=> /negP H; rewrite not_in_deref_V//=.
-    by apply/negP.
-  by rewrite disjointUr => /andP[H1 H2]; rewrite Ha//Hf//.
-Qed.
-
-(* Lemma deref2 s t:
-  acyclic_sigma s -> deref s (deref s t) = deref s t.
-Proof.
-  move=> H; elim: t => //=[v|f -> a ->]//.
-  case: fndP => //= vs; last by rewrite not_fnd//.
-  have: fdisjoint (domf s) (vars s.[vs]).
-    by apply/disjoint_sub/codom_vars_sub/H.
-  by apply/deref_disj_id.
-Qed. *)
-
-End s.
