theories/tree_test.v
@@ -103,10 +103,9 @@ Section Test1.
       rewrite [fresh_rules _ _]/= /fresh_rule !simpl_set.
       rewrite/rename [fresh_tm _ _ _]/= !simpl_set.
       rewrite /= !simpl_set /rename/= !simpl_set !inE /=.
-      move=> //.
+      by rewrite !unify_V_0r//=.
     by [].
     set R := (_ `|` _).
-    rewrite cat0f.
     apply: StepT => //.
       rewrite/step/=.
       rewrite/bc /next_subst [next _ _]/= acyclic_sigma_set_D//.
@@ -115,8 +114,9 @@ Section Test1.
       rewrite /fresh_rule/= !simpl_set.
       rewrite/rename [fresh_tm _ _ _]/= !simpl_set.
       rewrite !inE/= !simpl_set.
-      rewrite/deref/= !simpl_set/= !FmapE.fmapE/= eqxx/=.
-      rewrite unify_diff_ground//.
+      rewrite /=in_fnd/=?inE// => KK.
+      rewrite ffunE/= eqxx.
+      rewrite unify_ground//.
     by [].
     rewrite !simpl_set fsetUC.
     set T := (_ `|` _).
@@ -124,13 +124,10 @@ Section Test1.
     apply: StepT => //=.
       rewrite /bc [flatten_term _]/= [get_tm_hd _]/=.
       rewrite/next_subst/= acyclic_sigma_set_D//=.
-      rewrite deref_App//= deref_P//=.
       rewrite !FmapE.fmapE/= !simpl_set.
       rewrite/= /fresh_rule/= !simpl_set.
       rewrite /rename/= !simpl_set in_fset1/=.
-      rewrite !simpl_set.
-      rewrite/deref/= !simpl_set/= !FmapE.fmapE/= eqxx/=.
-      by rewrite unify_refl.
+      rewrite eqxx/= unify_ground//.
     by [].
     rewrite !simpl_set/=.
     apply: StopT => //=.
@@ -164,8 +161,8 @@ Section Test5.
     apply: StepT => //=.
       rewrite/bc [flatten_term _]/= [get_tm_hd _]/=.
       cbn iota.
-      rewrite /=!FmapE.fmapE eqxx/= !cat0f !simpl_set/=.
-      by [].
+      rewrite !FmapE.fmapE/= not_fnd//= unify_V_0r//=.
+      rewrite unify_V_0r//= acyclic_sigma0//=.
     by [].
     apply/StepT => //=.
     apply/StopT => //=.
@@ -196,9 +193,7 @@ Section Test6.
     set X:= (_ `|` _).
     apply: StepT => //=.
       rewrite/bc [flatten_term _]/= [get_tm_hd _]/=.
-      cbn iota.
-      rewrite !FmapE.fmapE eqxx/= !cat0f !simpl_set/=.
-      by [].
+      rewrite acyclic_sigma0/= !FmapE.fmapE/= not_fnd//= !unify_V_0r//=.
     by [].
     rewrite /varsU_rule/varsU_rhead/varsU_rprem/=/vars_atoms/= !simpl_set/=.
     set Y := _ `|` _.
